Add chase lev in a broken state, add invariants

ARMv8_Comp.thy
@@ -4,19 +4,22 @@ begin
 
 chapter \<open>ARMv8 Composition Theory\<close>
 
-definition local_op :: "('v,'r,'a) tstate_scheme \<Rightarrow> ('v,'r,'a) tstate_scheme \<Rightarrow> ('v,'r,'a) tstate_scheme"
-  where "local_op g lcl \<equiv>  g\<lparr> rg := rg lcl \<rparr>"
+type_synonym ('v,'r,'a) thread = "(('v,'a) grel \<times> ('v,'a) grel \<times> ('v,'r,'a) pred \<times> ('v,'r,'a) pred \<times> ('v,'r,'a) com_armv8 \<times> ('v,'r,'a) pred)"
+type_synonym ('v,'r,'a) threads = "('v,'r,'a) thread list"
+
+definition set_rg :: "('v,'r,'a) tstate \<Rightarrow> ('v,'r,'a) tstate \<Rightarrow> ('v,'r,'a) tstate"
+  where "set_rg g lcl \<equiv> g\<lparr> rg := rg lcl \<rparr>"
 
 definition ARMThread
-  where "ARMThread c = Thread local_op (lift\<^sub>c c)"
+  where "ARMThread c = Thread set_rg (lift\<^sub>c c)"
 
 lemma thr\<^sub>R [simp]:
-  "thr\<^sub>R local_op (step\<^sub>R R) = step R"
-  unfolding thr\<^sub>R_def step\<^sub>R_def step_def local_op_def by auto
+  "thr\<^sub>R set_rg \<langle>step\<^sub>t R\<rangle> = \<langle>step R\<rangle>"
+  unfolding thr\<^sub>R_def step\<^sub>t_def step_def set_rg_def by auto
 
 lemma thr\<^sub>G [simp]:
-  "thr\<^sub>G local_op (step G) = step G"
-  unfolding thr\<^sub>G_def step_def local_op_def by auto
+  "thr\<^sub>G set_rg \<langle>step G\<rangle> = \<langle>step G\<rangle>"
+  unfolding thr\<^sub>G_def step_def set_rg_def by auto
 
 definition univL
   where "univL P \<equiv> (\<lambda>m. \<forall>l. P (m\<lparr> rg := l \<rparr>))"
@@ -24,73 +27,98 @@ definition univL
 definition exL
   where "exL P \<equiv> (\<lambda>m. \<exists>l. P (m\<lparr> rg := l \<rparr>))"
 
-lemma [simp]:
-  "thr\<^sub>Q local_op (Collect Q) = Collect (exL Q)"
-  unfolding exL_def local_op_def thr\<^sub>Q_def by auto
+definition inv2
+  where "inv2 I \<equiv> \<lambda>(m,m'). \<forall>l. I (set_glb l m) \<longrightarrow> I (set_glb l m')"
 
 lemma [simp]:
-  "thr\<^sub>A local_op (Collect P) = Collect (univL P)"
-  unfolding univL_def local_op_def thr\<^sub>A_def by auto
+  "thr\<^sub>Q set_rg (Collect Q) = Collect (exL Q)"
+  unfolding exL_def set_rg_def thr\<^sub>Q_def
+  by auto (metis tstate_rec.select_convs(1))
+
+lemma [simp]:
+  "thr\<^sub>A set_rg (Collect P) = Collect (univL P)"
+  unfolding univL_def set_rg_def thr\<^sub>A_def
+  by auto (metis tstate_rec.select_convs(1))
 
 lemma armv8_thread:
-  assumes "guar\<^sub>c c G" "wellformed R G Q" "inter (step\<^sub>R R) (step G) (lift\<^sub>c c)" "P \<turnstile>\<^sub>p wp R G c Q"
-  shows "step R,step G \<turnstile> Collect (univL P) {ARMThread c} Collect (exL Q)"
+  assumes "guar\<^sub>c c (inv I \<and>\<^sub>p G)" "wellformed R G" "stable\<^sub>t R Q" "inter \<langle>step\<^sub>t (inv I \<and>\<^sub>p R)\<rangle> \<langle>step (inv I \<and>\<^sub>p G)\<rangle> (lift\<^sub>c c)" "P \<turnstile>\<^sub>p wp R c Q"
+  shows "\<langle>step (inv I \<and>\<^sub>p R)\<rangle>,\<langle>step (inv I \<and>\<^sub>p G)\<rangle> \<turnstile> \<langle>all\<^sub>t I \<and>\<^sub>p univL P\<rangle> {ARMThread c} \<langle>all\<^sub>t I \<and>\<^sub>p exL Q\<rangle>"
 proof -
-  have a: "R,G \<turnstile>\<^sub>s wp R G c Q {c} Q" using assms wp_valid unfolding valid_def by blast
-  have "step R,step G \<turnstile> Collect (univL (wp R G c Q)) {ARMThread c} Collect (exL Q)"
-    using rules.thread[OF a assms(3), of local_op] by (simp add: ARMThread_def)
-  thus ?thesis
-    apply (rule rules.conseq)
-    using assms(4) by (auto simp: univL_def pred_defs)
+  have a: "R,G,I \<turnstile>\<^sub>s wp R c Q {c} Q" using assms com_wp unfolding valid_def by blast
+  have "\<langle>step (inv I \<and>\<^sub>p R)\<rangle>,\<langle>step (inv I \<and>\<^sub>p G)\<rangle> \<turnstile> \<langle>all\<^sub>t I \<and>\<^sub>p univL (wp R c Q)\<rangle> {ARMThread c} \<langle>all\<^sub>t I \<and>\<^sub>p exL Q\<rangle>"
+    using rules.thread[OF a assms(4), of set_rg] by (simp add: ARMThread_def)
+  thus ?thesis by (rule rules.conseq) (insert assms(5), auto simp: univL_def )
 qed
 
-type_synonym ('v,'r,'a) thread = "(('v,'a) rpred \<times> ('v,'a) rpred \<times> ('v,'r,'a) pred \<times> ('v,'r,'a) lang \<times> ('v,'r,'a) pred)"
-type_synonym ('v,'r,'a) threads = "('v,'r,'a) thread list"
+section \<open>Parallel Composition Rules\<close>
 
+text \<open>Parallel composition of post-conditions\<close>
 fun Qs :: "('v,'r,'a) threads \<Rightarrow> ('v,'r,'a) pred"
   where 
     "Qs [] = (\<lambda>m. True)" | 
-    "Qs ((R,G,P,c,Q)#t) = (Qs t \<and>\<^sub>p exL Q)"
+    "Qs ((R,G,I,P,c,Q)#t) = (Qs t \<and>\<^sub>p exL Q)"
 
+text \<open>Parallel composition of pre-conditions\<close>
 fun Ps :: "('v,'r,'a) threads \<Rightarrow>('v,'r,'a) pred"
   where 
     "Ps [] = (\<lambda>m. True)" | 
-    "Ps ((R,G,P,c,Q)#t) = (Ps t \<and>\<^sub>p univL P)"
+    "Ps ((R,G,I,P,c,Q)#t) = (Ps t \<and>\<^sub>p univL P)"
 
-fun Rs :: "('v,'r,'a) threads \<Rightarrow> ('v,'a) rpred"
+text \<open>Parallel composition of rely specification\<close>
+fun Rs :: "('v,'r,'a) threads \<Rightarrow> ('v,'r,'a) trel"
   where
     "Rs [] = (\<lambda>m. True)" |
-    "Rs ((R,G,c,Q)#t) = (Rs t \<and>\<^sub>p R)"
+    "Rs ((R,G,c,Q)#t) = (Rs t \<and>\<^sub>p step R)"
 
-fun Gs :: "('v,'r,'a) threads \<Rightarrow> ('v,'a) rpred"
+text \<open>Parallel composition of guarantee specification\<close>
+fun Gs :: "('v,'r,'a) threads \<Rightarrow> ('v,'r,'a) trel"
   where
     "Gs [] = (\<lambda>m. False)" |
-    "Gs ((R,G,c,Q)#t) = (Gs t \<or>\<^sub>p G)"
+    "Gs ((R,G,c,Q)#t) = (Gs t \<or>\<^sub>p step G)"
 
-fun Cs :: "('v,'r,'a) threads \<Rightarrow> (('v,'r,'a) inst,('v,'r,'a) tstate_scheme) com"
+text \<open>Parallel composition of a list of programs\<close>
+fun Cs :: "('v,'r,'a) threads \<Rightarrow> (('v,'r,'a) auxop,('v,'r,'a) tstate) com"
   where 
     "Cs [] = undefined " |
-    "Cs [(R,G,P,c,Q)] = ARMThread c" |
+    "Cs [(R,G,I,P,c,Q)] = ARMThread c" |
     "Cs (c#ts) = Cs [c] || Cs ts"
 
-definition wfs :: "('v,'r,'a) threads \<Rightarrow> bool"
-  where "wfs t \<equiv> \<forall>(R,G,P,c,Q) \<in> set t. 
-                  wellformed R G Q \<and> 
-                  guar\<^sub>c c G \<and> 
-                  inter (step\<^sub>R R) (step G) (lift\<^sub>c c) \<and>
-                  (P \<turnstile>\<^sub>p wp R G c Q)"
+text \<open>Parallel composition of a list of programs\<close>
+fun Is :: "('v,'r,'a) threads \<Rightarrow> ('v,'a) gpred"
+  where 
+    "Is [] = (\<lambda>m. True)" | 
+    "Is ((R,G,I,P,c,Q)#t) = (Is t \<and>\<^sub>p I)"
 
+text \<open>Properties required for each thread\<close>
+definition local_props :: "('v,'r,'a) threads \<Rightarrow> bool"
+  where "local_props t \<equiv> \<forall>(R,G,I,P,c,Q) \<in> set t. 
+            stable\<^sub>t R Q \<and> wellformed R G \<and> 
+            guar\<^sub>c c (inv2 I \<and>\<^sub>p G) \<and> (P \<turnstile>\<^sub>p wp R c Q) \<and> 
+            inter \<langle>step\<^sub>t (inv2 I \<and>\<^sub>p R)\<rangle> \<langle>step (inv2 I \<and>\<^sub>p G)\<rangle> (lift\<^sub>c c)"
+
+text \<open>Rely/guarantee compatibility for a list of threads\<close>
 definition rg_comp :: "('v,'r,'a) threads \<Rightarrow> bool"
-  where "rg_comp t \<equiv> \<forall>i j. i < length t \<longrightarrow> j < length t \<longrightarrow> i \<noteq> j \<longrightarrow> fst (snd (t ! i)) \<turnstile>\<^sub>p fst (t ! j)"
+  where "rg_comp t \<equiv> 
+            \<forall>i j. i < length t \<longrightarrow> j < length t \<longrightarrow> i \<noteq> j \<longrightarrow> fst (snd (t ! i)) \<turnstile>\<^sub>p fst (t ! j)"
 
+subsection \<open>Composition Properties\<close>
+
+text \<open>Subset of compositional threads are compositional\<close>
 lemma rg_comp_tailI:
-  "rg_comp (a#t) \<Longrightarrow> rg_comp t"
-  unfolding rg_comp_def apply auto
-  by (metis (no_types, lifting) Ex_less_Suc Suc_inject less_trans_Suc nth_Cons_Suc)
+  assumes "rg_comp (s#t)" 
+  shows "rg_comp t"
+proof (clarsimp simp: rg_comp_def)
+  fix i j a b
+  assume "i < length t" "j < length t" "i \<noteq> j" "fst (snd (t ! i)) (a, b)" 
+  hence "Suc i < length (s#t)" "Suc j < length (s#t)" 
+        "Suc i \<noteq> Suc j" "fst (snd ((s#t) ! Suc i)) (a, b)"  by auto
+  hence "fst ((s#t) ! Suc j) (a, b)" using assms unfolding rg_comp_def by blast
+  thus "fst (t ! j) (a, b)" by auto
+qed
 
 lemma Gs_rel:
-  assumes "\<forall>i. i < length t \<longrightarrow> step (fst (snd ((t :: ('v,'r,'a) threads) ! i))) \<subseteq> ((step R) :: ('v,'r,'a) tstate_scheme rel)"
-  shows "step (Gs t) \<subseteq> step R"
+  assumes "\<forall>i. i < length t \<longrightarrow> step (fst (snd ((t :: ('v,'r,'a) threads) ! i))) \<turnstile>\<^sub>p (step R :: ('v,'r,'a) trel)"
+  shows "\<langle>Gs t\<rangle> \<subseteq> \<langle>step R\<rangle>"
   using assms
 proof (induct t)
   case Nil
@@ -98,13 +126,13 @@ proof (induct t)
 next
   case (Cons a t)
   obtain R' G c Q where a [simp]: "a = (R',G,c,Q)" by (cases a, auto)
-  have i: "\<And>i. i < length (a # t) \<Longrightarrow> step (fst (snd ((a # t) ! i))) \<subseteq> ((step R) :: ('v,'r,'a) tstate_scheme rel)"
+  have i: "\<And>i. i < length (a # t) \<Longrightarrow> step (fst (snd ((a # t) ! i))) \<turnstile>\<^sub>p ((step R) :: ('v,'r,'a) trel)"
     using Cons(2) by auto
 
-  have b: "\<forall>i. i <length t \<longrightarrow> step (fst (snd (t ! i))) \<subseteq> ((step R) :: ('v,'r,'a) tstate_scheme rel)" 
-          "step G \<subseteq> ((step R) :: ('v,'r,'a) tstate_scheme rel)"
+  have b: "\<forall>i. i <length t \<longrightarrow> step (fst (snd (t ! i))) \<turnstile>\<^sub>p ((step R) :: ('v,'r,'a) trel)" 
+          "step G \<turnstile>\<^sub>p ((step R) :: ('v,'r,'a) trel)"
     apply (intro allI impI)
-    apply (subgoal_tac "step (fst (snd ((a # t) ! Suc i))) \<subseteq> step R")
+    apply (subgoal_tac "step (fst (snd ((a # t) ! Suc i))) \<turnstile>\<^sub>p step R")
     apply auto[1]
     apply (rule i)
     apply auto
@@ -112,14 +140,12 @@ next
     apply auto
     done
 
-  show ?case using Cons(1)[OF b(1)] b(2)
-    apply (auto simp: step_def pred_defs)
-    sorry
+  show ?case using Cons(1)[OF b(1)] b(2) by (auto simp: step_def pred_defs)
 qed
 
 lemma Rs_rel:
-  assumes "\<forall>i. i < length t \<longrightarrow> (step G  :: ('v,'r,'a) tstate_scheme rel) \<subseteq> step (fst ( ((t :: ('v,'r,'a) threads) ! i)))"
-  shows "step G \<subseteq> step (Rs t)"
+  assumes "\<forall>i. i < length t \<longrightarrow> (step G  :: ('v,'r,'a) trel) \<turnstile>\<^sub>p step (fst ( ((t :: ('v,'r,'a) threads) ! i)))"
+  shows "\<langle>step G\<rangle> \<subseteq> \<langle>Rs t\<rangle>"
   using assms
 proof (induct t)
   case Nil
@@ -127,81 +153,74 @@ proof (induct t)
 next
   case (Cons a t)
   obtain R G' c Q where a [simp]: "a = (R,G',c,Q)" by (cases a, auto)
-  have i: "\<And>i. i < length (a # t) \<Longrightarrow> ((step G) :: ('v,'r,'a) tstate_scheme rel) \<subseteq> step  (fst ((a # t) ! i))"
+  have i: "\<And>i. i < length (a # t) \<Longrightarrow> ((step G) :: ('v,'r,'a) trel) \<turnstile>\<^sub>p step  (fst ((a # t) ! i))"
     using Cons(2) by auto
 
-  have b: "\<forall>i. i <length t \<longrightarrow> ((step G) :: ('v,'r,'a) tstate_scheme rel) \<subseteq> step  (fst (t ! i))"
-          "step G \<subseteq> ((step R) :: ('v,'r,'a) tstate_scheme rel)"
+  have b: "\<forall>i. i <length t \<longrightarrow> ((step G) :: ('v,'r,'a) trel) \<turnstile>\<^sub>p step  (fst (t ! i))"
+          "step G \<turnstile>\<^sub>p ((step R) :: ('v,'r,'a) trel)"
     apply (intro allI impI)
-    using i apply force using i by force
+    using i 
+    apply (metis (no_types, hide_lams) length_Suc_conv not_less_eq nth_Cons_Suc)
+    using i[of 0] by auto
 
-  show ?case using Cons(1)[OF b(1)] b(2)
-    apply (auto simp: step_def pred_defs)
-    sorry
+  show ?case using Cons(1)[OF b(1)] b(2) by (auto simp: step_def pred_defs)
 qed
 
 lemma rg_comp_Gs:
-  assumes "rg_comp ((R,G,P,c,Q)#t)" 
-  shows "step (Gs t) \<subseteq> step R"
+  assumes "rg_comp ((R,G,I,P,c,Q)#t)" 
+  shows "\<langle>Gs t\<rangle> \<subseteq> \<langle>step R\<rangle>"
 proof -
   have "\<forall>i. i < length t \<longrightarrow> fst (snd (t ! i)) \<turnstile>\<^sub>p R"
-    using assms unfolding rg_comp_def sorry
-  hence "\<forall>i. i < length t \<longrightarrow> step (fst (snd (t ! i))) \<subseteq> step R"
-    unfolding step_def pred_defs by auto
+    using assms unfolding rg_comp_def
+    by (metis (no_types, lifting) Suc_mono fst_conv length_Cons length_greater_0_conv list.distinct(1) list.sel(3) nat.simps(3) nth_Cons_0 nth_tl)
+  hence "\<forall>i. i < length t \<longrightarrow> step (fst (snd (t ! i))) \<turnstile>\<^sub>p step R"
+    unfolding step_def by auto
   thus ?thesis using Gs_rel by blast
 qed
 
 lemma rg_comp_Rs:
-  assumes "rg_comp ((R,G,P,c,Q)#t)" 
-  shows "step G \<subseteq> step (Rs t)"
+  assumes "rg_comp ((R,G,I,P,c,Q)#t)" 
+  shows "\<langle>step G\<rangle> \<subseteq> \<langle>Rs t\<rangle>"
 proof -
   have "\<forall>i. i < length t \<longrightarrow> G \<turnstile>\<^sub>p fst (t ! i)"
-    using assms unfolding rg_comp_def by force
-  hence "\<forall>i. i < length t \<longrightarrow> step G \<subseteq> step (fst (t ! i))"
+    using assms unfolding rg_comp_def 
+    by (metis (no_types, lifting) Suc_mono fst_conv length_Cons length_greater_0_conv list.distinct(1) list.sel(3) nat.simps(3) nth_Cons_0 nth_tl snd_conv)
+  hence "\<forall>i. i < length t \<longrightarrow> step G \<turnstile>\<^sub>p step (fst (t ! i))"
     unfolding step_def pred_defs by auto
   thus ?thesis using Rs_rel by blast
 qed
 
 lemma armv8_parallel:
-  assumes "length t \<noteq> 0" "wfs t" "rg_comp t"
-  shows "step (Rs t), step (Gs t) \<turnstile> Collect (Ps t) {Cs t} Collect (Qs t)"
+  assumes "length t \<noteq> 0" "local_props t" "rg_comp t"
+  shows "\<langle>Rs t\<rangle>, \<langle>Gs t\<rangle> \<turnstile> \<langle>Ps t\<rangle> {Cs t} \<langle>Qs t\<rangle>"
   using assms
 proof (induct t)
   case (Cons a t)
-  obtain R G P c Q where a [simp]: "a = (R,G,P,c,Q)" by (cases a, auto)
-  have wf: "guar\<^sub>c c G" "wellformed R G Q" 
-           "inter (step\<^sub>R R) (step G) (lift\<^sub>c c)" "wfs t"
-           "P \<turnstile>\<^sub>p  wp R G c Q"
-    using Cons(3) by (auto simp: wfs_def)
-  have j: "step R,step G \<turnstile> Collect (univL P) {ARMThread c} Collect (exL Q)" 
-    using armv8_thread[OF wf(1,2,3,5)] by blast
-  have c: "step (Gs t) \<subseteq> step R" "step G \<subseteq> step (Rs t)"
-    using rg_comp_Rs rg_comp_Gs Cons sorry (* apply fastforce
-    using rg_comp_Rs rg_comp_Gs Cons apply fastforce
-    done *)
+  obtain R G I P c Q where a [simp]: "a = (R,G,I,P,c,Q)" by (cases a, auto)
+  have wf: 
+      "guar\<^sub>c c (inv I \<and>\<^sub>p G)" "wellformed R G" "stable\<^sub>t R Q" 
+      "inter \<langle>step\<^sub>t (inv I \<and>\<^sub>p R)\<rangle> \<langle>step (inv I \<and>\<^sub>p G)\<rangle> (lift\<^sub>c c)" 
+      "P \<turnstile>\<^sub>p wp R c Q" "local_props t"
+    using Cons(3) by (auto simp: local_props_def)
+  have j: "\<langle>step (inv I \<and>\<^sub>p R)\<rangle>,\<langle>step (inv I \<and>\<^sub>p G)\<rangle> \<turnstile> \<langle>all\<^sub>t I \<and>\<^sub>p univL P\<rangle> {ARMThread c} \<langle>all\<^sub>t I \<and>\<^sub>p exL Q\<rangle>" 
+    using armv8_thread[OF wf(1,2,3,4,5)] by blast
+  have c: "\<langle>Gs t\<rangle> \<subseteq> \<langle>step R\<rangle>" "\<langle>step G\<rangle> \<subseteq> \<langle>Rs t\<rangle>"
+    using rg_comp_Rs[of _ _ I P] rg_comp_Gs[of _ _ I P] Cons by auto
   show ?case 
   proof (cases "t = []")
     case True
-    then show ?thesis using j by (auto simp: exL_def pred_defs)
+    then show ?thesis using j by (auto simp: exL_def)
   next
     case False
-    hence t: "step (Rs t),step (Gs t) \<turnstile> Collect (Ps t) {Cs t} Collect (Qs t)" 
-      using Cons wf(4) rg_comp_tailI by blast
-    have [simp]: "Cs ((R, G, P, c, Q) # t) = ARMThread c || Cs t" using False by (cases t) auto
-    show ?thesis
-      apply clarsimp
-      apply (rule rules.conseq[OF rules.par[OF j t c]])
-      by (auto simp: step_def o_def exL_def pred_defs)
+    hence t: "\<langle>Rs t\<rangle>, \<langle>Gs t\<rangle> \<turnstile> \<langle>Ps t\<rangle> {Cs t} \<langle>Qs t\<rangle>" using Cons wf(6) rg_comp_tailI sorry
+    have [simp]: "Cs ((R, G, I, P, c, Q) # t) = ARMThread c || Cs t" using False by (cases t) auto
+    show ?thesis by (clarsimp, rule rules.conseq[OF rules.par[OF j t c]]) auto
   qed
 qed auto
 
 lemma armv8_sound:
-  assumes "length t \<noteq> 0" "wfs t" "rg_comp t"
-  shows "validity (Cs t) (Collect (Ps t)) (step (Rs t)) (step (Gs t)) (Collect (Qs t))"
-proof -
-  have "step (Rs t), step (Gs t) \<turnstile> Collect (Ps t) {Cs t} Collect (Qs t)"
-    using assms armv8_parallel by auto
-  thus ?thesis by (rule sound)
-qed
+  assumes "length t \<noteq> 0" "local_props t" "rg_comp t"
+  shows "validity (Cs t) \<langle>Ps t\<rangle> \<langle>Rs t\<rangle> \<langle>Gs t\<rangle> \<langle>Qs t\<rangle>"
+  using assms by (intro sound armv8_parallel) auto
 
 end
