ARMv8_Rules.thy
@@ -1,668 +1,463 @@
 theory ARMv8_Rules
-  imports Soundness ARMv8
+  imports Soundness ARMv8 "HOL-Eisbach.Eisbach"
 begin
-
-section \<open>Predicate Transformations\<close>
-
-definition glb :: "('v,'r,'a) tstate_scheme \<Rightarrow> ('v,'a) gstate_scheme"
-  where "glb m \<equiv> \<lparr> st = st m, \<dots> = more m \<rparr>"
-
-definition set_glb :: "('v,'r,'a) tstate_scheme \<Rightarrow> ('v,'a) gstate_scheme \<Rightarrow> ('v,'r,'a) tstate_scheme"
-  where "set_glb m g \<equiv> \<lparr> st = st g, rg = rg m, \<dots> = gstate.more g \<rparr>"
-
-definition stabilize :: "('v,'a) rpred \<Rightarrow> ('v,'r,'a) pred \<Rightarrow> ('v,'r,'a) pred"
-  where "stabilize R P \<equiv> \<lambda>m. \<forall>g. R (glb m,g) \<longrightarrow> P (set_glb m g)"
-
-definition aux_upd
-  where "aux_upd a \<equiv> \<lambda>m. m\<lparr>tstate.more := a m\<rparr>"
-
-text \<open>Transform a predicate based on an instruction\<close>
-fun wp\<^sub>i :: "('v,'r,'a) inst \<Rightarrow> ('v,'r,'a) pred \<Rightarrow> ('v,'r,'a) pred" 
-  where 
-    "wp\<^sub>i (load v e a) Q = (\<lambda>m. st m v = ev (rg m) e \<longrightarrow> Q (aux_upd a m))" | 
-    "wp\<^sub>i (store v e a) Q = (\<lambda>m. Q (aux_upd a (m(v :=\<^sub>s ev (rg m) e))))" | 
-    "wp\<^sub>i (op r e) Q = (\<lambda>m. Q (m (r :=\<^sub>r ev (rg m) e)))" |
-    "wp\<^sub>i (cmp e\<^sub>1 f e\<^sub>2) Q = (\<lambda>m. f (ev (rg m) e\<^sub>1) (ev (rg m) e\<^sub>2) \<longrightarrow> Q m)" | 
-    "wp\<^sub>i (cas\<^sub>T v e\<^sub>1 e\<^sub>2 a) Q = (\<lambda>m. st m v = ev (rg m) e\<^sub>1 \<longrightarrow> Q (aux_upd a (m(v :=\<^sub>s ev (rg m) e\<^sub>2))))" | 
-    "wp\<^sub>i (cas\<^sub>F v e\<^sub>1 e\<^sub>2 a) Q = (\<lambda>m. st m v \<noteq> ev (rg m) e\<^sub>1 \<longrightarrow> Q (aux_upd a m))" | 
-    "wp\<^sub>i _ Q = Q"
-
-fun guar\<^sub>i
-  where
-    "guar\<^sub>i (load v e a) G = (\<lambda>m. st m v = ev (rg m) e \<longrightarrow> G (glb m,glb (aux_upd a m)))" |
-    "guar\<^sub>i (store v e a) G = (\<lambda>m. G (glb m,glb (aux_upd a (m(v :=\<^sub>s ev (rg m) e)))))" |
-    "guar\<^sub>i (cas\<^sub>T v e\<^sub>1 e\<^sub>2 a) G = 
-      (\<lambda>m. st m v = ev (rg m) e\<^sub>1 \<longrightarrow> G (glb m,glb (aux_upd a (m(v :=\<^sub>s ev (rg m) e\<^sub>2)))))" | 
-    "guar\<^sub>i (cas\<^sub>F v e\<^sub>1 e\<^sub>2 a) G = 
-      (\<lambda>m. st m v \<noteq> ev (rg m) e\<^sub>1 \<longrightarrow> G (glb m,glb (aux_upd a m)))" | 
-    "guar\<^sub>i _ _ = (\<lambda>m. True)"
-
-definition step\<^sub>R :: "('v,'a) rpred \<Rightarrow> ('v,'r,'a) tstate_scheme rel"
-  where "step\<^sub>R R \<equiv> {(m,m'). R (glb m, glb m') \<and> rg m = rg m'}"
-
-definition step :: "('v,'a) rpred \<Rightarrow> ('v,'r,'a) tstate_scheme rel"
-  where "step R \<equiv> {(m,m'). R (glb m, glb m')}"
-
-text \<open>The WP predicate transformer given a rely R and guarantee G\<close>
-fun wp :: "('v,'a) rpred \<Rightarrow> ('v,'a) rpred \<Rightarrow> ('v,'r,'a) lang \<Rightarrow> ('v,'r,'a) pred \<Rightarrow> ('v,'r,'a) pred"
-  where
-    "wp R G Skip Q = Q" |
-    "wp R G Fence Q = Q" |
-    "wp R G (Load v r\<^sub>a r a) Q = stabilize R (v \<and>\<^sub>p (\<lambda>m. Q (aux_upd a (m (r :=\<^sub>r st m (rg m r\<^sub>a))))))" |
-    "wp R G (Store v r\<^sub>a r a) Q = stabilize R (v \<and>\<^sub>p (\<lambda>m. Q (aux_upd a (m (rg m r\<^sub>a :=\<^sub>s rg m r)))))" |
-    "wp R G (Op r e) Q = wp\<^sub>i (op r e) Q" |
-    "wp R G (Test p) Q = stabilize R (p \<longrightarrow>\<^sub>p Q)" |
-    "wp R G (Assert p) Q = (stabilize R p \<and>\<^sub>p Q)" |
-    "wp R G (CAS v r\<^sub>a r\<^sub>1 r\<^sub>2 r T F a) Q = 
-      stabilize R (
-        v \<and>\<^sub>p 
-        (\<lambda>m. st m (rg m r\<^sub>a) = rg m r\<^sub>1 \<longrightarrow> Q (aux_upd a (m(rg m r\<^sub>a :=\<^sub>s rg m r\<^sub>2, r :=\<^sub>r T)))) \<and>\<^sub>p 
-        (\<lambda>m. st m (rg m r\<^sub>a) \<noteq> rg m r\<^sub>1 \<longrightarrow> Q (aux_upd a (m(r :=\<^sub>r F)))))" |
-    "wp R G (Seq c\<^sub>1 c\<^sub>2) Q = wp R G c\<^sub>1 (wp R G c\<^sub>2 Q)" |
-    "wp R G (If e\<^sub>1 f e\<^sub>2 c\<^sub>1 c\<^sub>2) Q = (
-      wp\<^sub>i (cmp e\<^sub>1 f e\<^sub>2) (wp R G c\<^sub>1 Q) \<and>\<^sub>p wp\<^sub>i (ncmp e\<^sub>1 f e\<^sub>2) (wp R G c\<^sub>2 Q))" |
-    "wp R G (While e\<^sub>1 f e\<^sub>2 I c) Q = 
-      (stabilize R I \<and>\<^sub>p assert (
-        I \<turnstile>\<^sub>p wp\<^sub>i (cmp e\<^sub>1 f e\<^sub>2) (wp R G c (stabilize R I)) \<and>\<^sub>p wp\<^sub>i (ncmp e\<^sub>1 f e\<^sub>2) Q))" |
-    "wp R G (DoWhile I c e\<^sub>1 f e\<^sub>2) Q = 
-      (stabilize R I \<and>\<^sub>p assert (
-        I \<turnstile>\<^sub>p wp R G c (wp\<^sub>i (cmp e\<^sub>1 f e\<^sub>2) (stabilize R I) \<and>\<^sub>p wp\<^sub>i (ncmp e\<^sub>1 f e\<^sub>2) Q)))"
 
 section \<open>Wellformedness\<close>
 
-text \<open>Couple all wellformedness conditions into a single definition\<close>
-definition wellformed :: "('v,'a) rpred \<Rightarrow> ('v,'a) rpred \<Rightarrow> ('v,'r,'a) pred \<Rightarrow> bool"
-  where "wellformed R G Q \<equiv> 
-    stable (step\<^sub>R R) (Collect Q) \<and> reflexive R \<and> transitive R \<and> reflexive G" 
+text \<open>
+Abstract theory is in terms of sets of states, where as the WP reasoning uses functions.
+This lifting converts to the abstract.
+\<close>
+abbreviation lift_encoding ("\<langle>_\<rangle>" 1000) 
+  where "lift_encoding \<equiv> Collect"
 
-text \<open>Establish wellformedness of a false predicate\<close>
-lemma wf_false:
-  "\<forall>m. \<not> P m \<Longrightarrow> wellformed R G Q \<Longrightarrow> wellformed R G P"
-  unfolding wellformed_def stable_def by (auto)
+text \<open>Lift an invariant to a relation\<close>
+definition inv :: "(('v,'a) gstate \<Rightarrow> bool) \<Rightarrow> ('v,'a) grel"
+  where "inv I \<equiv> \<lambda>(m,m'). I m \<longrightarrow> I m'"
+
+text \<open>Convert a global predicate into a thread local predicate by ignoring the local state\<close>
+definition all\<^sub>t :: "(('v,'a) gstate \<Rightarrow> bool) \<Rightarrow> ('v,'r,'a) pred"
+  where "all\<^sub>t I \<equiv> \<lambda>m. I (glb m)"
+
+text \<open>Lift a relational predicate with no constraint on thread state\<close>
+definition step :: "('v,'a) grel \<Rightarrow> ('v,'r,'a) trel"
+  where "step R \<equiv> \<lambda>(m,m'). R (glb m, glb m')"
+
+text \<open>Lift a relational predicate and assume it preserves the thread state\<close>
+definition step\<^sub>t :: "('v,'a) grel \<Rightarrow> ('v,'r,'a) trel"
+  where "step\<^sub>t R \<equiv> \<lambda>(m,m'). R (glb m, glb m') \<and> rg m = rg m'"
+
+text \<open>Define stability in terms of a relational predicate that preserves the thread state\<close>
+abbreviation stable\<^sub>t
+  where "stable\<^sub>t R P \<equiv> stable \<langle>step\<^sub>t R\<rangle> \<langle>P\<rangle>"
+
+text \<open>Couple all wellformedness conditions into a single definition\<close>
+abbreviation wellformed :: "('v,'a) grel \<Rightarrow> ('v,'a) grel \<Rightarrow> bool"
+  where "wellformed R G \<equiv> reflexive R \<and> transitive R \<and> reflexive G" 
 
 text \<open>Show that a stabilized predicate is stable\<close>
 lemma stabilize_stable [intro]:
-  assumes wf: "wellformed R G P"
-  shows "stable (step\<^sub>R R) (Collect (stabilize R Q))"
-  unfolding stable_def step\<^sub>R_def
+  assumes wf: "wellformed R G"
+  shows "stable\<^sub>t R (stabilize R Q)"
+  unfolding stable_def step\<^sub>t_def
 proof (clarsimp)
   fix m m'
   assume a: "stabilize R Q m" "R (glb m, glb m')" "rg m = rg m'"
   have "\<forall>g''. R (glb m',g'') \<longrightarrow> R (glb m,g'')"
-    using assms a(2) unfolding wellformed_def transitive_def by blast
+    using assms a(2) unfolding transitive_def by blast
   thus "stabilize R Q m'" using a(1,3) by (auto simp: stabilize_def set_glb_def)
 qed
 
-text \<open>Stabilization preserves wellformedness\<close>
-lemma stabilize_wellformed [intro]:
-  assumes "wellformed R G P"
-  shows "wellformed R G (stabilize R Q)" (is "wellformed R G ?P")
-proof -
-  have "stable (step\<^sub>R R) (Collect ?P)" 
-    using stabilize_stable assms by blast
-  thus ?thesis using assms unfolding wellformed_def by blast
-qed
-
-lemma stable_conj [intro]:
-  assumes "stable R (Collect P)" "stable R (Collect Q)"
-  shows "stable R (Collect (P \<and>\<^sub>p Q))"
+text \<open>The conjunction of two stable predicates is stable\<close>
+lemma stable\<^sub>t_conj [intro]:
+  assumes "stable\<^sub>t R P" "stable\<^sub>t R Q"
+  shows "stable\<^sub>t R (P \<and>\<^sub>p Q)"
   using assms by (auto simp: stable_def pred_defs)
-
-lemma wellformed_conjI [intro]:
-  assumes "wellformed R G P" "wellformed R G Q"
-  shows "wellformed R G (P \<and>\<^sub>p Q)"
-  using assms by (auto simp: wellformed_def)
-
-lemma [simp]:
-  "set_glb m (glb m) = m"
-  by (auto simp: set_glb_def glb_def)
 
 text \<open>Elimination rule to ignore the stabilization process\<close>
 lemma stabilizeE:
   assumes "stabilize R P m"
-  assumes "wellformed R G Q"
+  assumes "wellformed R G"
   obtains "P m"
-  using assms unfolding wellformed_def reflexive_def stabilize_def sorry
+proof -
+  have "\<forall>g. R (glb m, g) \<longrightarrow> P (set_glb m g)" "R (glb m, glb m)"
+    using assms by (auto simp: reflexive_def stabilize_def)
+  thus ?thesis using that by auto
+qed
 
-section \<open>Program Wellformedness\<close>
+text \<open>Stabilization preserves entailment\<close>
+lemma stabilize_entail [intro!]:
+  assumes "wellformed R G"
+  assumes "P \<turnstile>\<^sub>p Q"
+  shows "stabilize R P \<turnstile>\<^sub>p Q"
+  using assms by (auto simp: pred_defs stabilize_def)
 
-text \<open>Ensure all operations have preconditions strong enough to discharge their guarantee\<close>
+section \<open>Predicate Transformations\<close>
+
+named_theorems wp_defs
+
+text \<open>Transform a predicate based on an sub-operation\<close>
+fun wp\<^sub>i :: "('v,'r) subop \<Rightarrow> ('v,'r,'a) trans" 
+  where 
+    "wp\<^sub>i (load v e) Q = (\<lambda>m. st m v = ev (rg m) e \<longrightarrow> Q m)" | 
+    "wp\<^sub>i (store v e) Q = (\<lambda>m. Q (m(v :=\<^sub>s ev (rg m) e)))" | 
+    "wp\<^sub>i (op r e) Q = (\<lambda>m. Q (m (r :=\<^sub>r ev (rg m) e)))" |
+    "wp\<^sub>i (cmp b) Q = (\<lambda>m. ev\<^sub>B (rg m) b \<longrightarrow> Q m)" | 
+    "wp\<^sub>i (cas\<^sub>T v e\<^sub>1 e\<^sub>2) Q = (\<lambda>m. st m v = ev (rg m) e\<^sub>1 \<longrightarrow> Q (m(v :=\<^sub>s ev (rg m) e\<^sub>2)))" | 
+    "wp\<^sub>i (cas\<^sub>F v e\<^sub>1 e\<^sub>2) Q = (\<lambda>m. st m v \<noteq> ev (rg m) e\<^sub>1 \<longrightarrow> Q m)" | 
+    "wp\<^sub>i _ Q = Q"
+
+text \<open>Transform a predicate based on an auxiliary state update\<close>
+fun wp\<^sub>a :: "('v,'r,'a) auxfn \<Rightarrow> ('v,'r,'a) trans"
+  where "wp\<^sub>a a Q = (\<lambda>m. Q (m(aux: a)))"
+
+text \<open>Transform a predicate based on a Load instruction\<close>
+definition wp_Load :: "('v,'r) exp \<Rightarrow> 'r \<Rightarrow> ('v,'r,'a) auxfn \<Rightarrow> ('v,'r,'a) trans"
+  where "wp_Load r\<^sub>a r a Q \<equiv> \<lambda>m. Q (m (r :=\<^sub>r st m (ev (rg m) r\<^sub>a), aux: a))"
+declare wp_Load_def [wp_defs]
+
+text \<open>Transform a predicate based on a Store instruction\<close>
+definition wp_Store :: "('v,'r) exp \<Rightarrow> 'r \<Rightarrow> ('v,'r,'a) auxfn \<Rightarrow> ('v,'r,'a) trans"
+  where "wp_Store r\<^sub>a r a Q \<equiv> \<lambda>m. Q (m (ev (rg m) r\<^sub>a :=\<^sub>s rg m r, aux: a))"
+declare wp_Store_def [wp_defs]
+
+text \<open>Transform a predicate based on a successful CAS instruction\<close>
+definition wp_CAS\<^sub>T :: "'r \<Rightarrow> 'r \<Rightarrow> 'r \<Rightarrow> 'r \<Rightarrow> 'v \<Rightarrow> 'v \<Rightarrow> ('v,'r,'a) auxfn \<Rightarrow> ('v,'r,'a) trans"
+  where "wp_CAS\<^sub>T r\<^sub>a r\<^sub>1 r\<^sub>2 r T F a Q \<equiv> 
+    \<lambda>m. st m (rg m r\<^sub>a) = rg m r\<^sub>1 \<longrightarrow> Q (m(rg m r\<^sub>a :=\<^sub>s rg m r\<^sub>2, r :=\<^sub>r T, aux: a))"
+declare wp_CAS\<^sub>T_def [wp_defs]
+
+text \<open>Transform a predicate based on a failed CAS instruction\<close>
+definition wp_CAS\<^sub>F :: "'r \<Rightarrow> 'r \<Rightarrow> 'r \<Rightarrow> 'r \<Rightarrow> 'v \<Rightarrow> 'v \<Rightarrow> ('v,'r,'a) auxfn \<Rightarrow> ('v,'r,'a) trans"
+  where "wp_CAS\<^sub>F r\<^sub>a r\<^sub>1 r\<^sub>2 r T F a Q \<equiv> 
+    \<lambda>m. st m (rg m r\<^sub>a) \<noteq> rg m r\<^sub>1 \<longrightarrow> Q (m(r :=\<^sub>r F, aux: a))"
+declare wp_CAS\<^sub>F_def [wp_defs]
+
+text \<open>Transform a predicate based on a CAS instruction\<close>
+definition wp_CAS :: "'r \<Rightarrow> 'r \<Rightarrow> 'r \<Rightarrow> 'r \<Rightarrow> 'v \<Rightarrow> 'v \<Rightarrow> ('v,'r,'a) auxfn \<Rightarrow> ('v,'r,'a) trans"
+  where "wp_CAS r\<^sub>a r\<^sub>1 r\<^sub>2 r T F a Q \<equiv> wp_CAS\<^sub>T r\<^sub>a r\<^sub>1 r\<^sub>2 r T F a Q \<and>\<^sub>p wp_CAS\<^sub>F r\<^sub>a r\<^sub>1 r\<^sub>2 r T F a Q"
+declare wp_CAS_def [wp_defs]
+
+text \<open>Transform a predicate based on a program c within an environment R\<close>
+fun wp :: "('v,'a) grel \<Rightarrow> ('v,'r,'a) com_armv8 \<Rightarrow> ('v,'r,'a) trans"
+  where
+    "wp R Skip Q = Q" |
+    "wp R Fence Q = Q" |
+    "wp R (Load v r\<^sub>a r a) Q = stabilize R (v \<and>\<^sub>p wp_Load r\<^sub>a r a Q)" |
+    "wp R (Store v r\<^sub>a r a) Q = stabilize R (v \<and>\<^sub>p wp_Store r\<^sub>a r a Q)" |
+    "wp R (Op r e) Q = wp\<^sub>i (op r e) Q" |
+    "wp R (Test p) Q = stabilize R (p \<longrightarrow>\<^sub>p Q)" |
+    "wp R (Assert p) Q = (stabilize R p \<and>\<^sub>p Q)" |
+    "wp R (CAS v r\<^sub>a r\<^sub>1 r\<^sub>2 r T F a) Q = stabilize R (v \<and>\<^sub>p wp_CAS r\<^sub>a r\<^sub>1 r\<^sub>2 r T F a Q)" |
+    "wp R (Seq c\<^sub>1 c\<^sub>2) Q = wp R c\<^sub>1 (wp R c\<^sub>2 Q)" |
+    "wp R (If b c\<^sub>1 c\<^sub>2) Q = (wp\<^sub>i (cmp b) (wp R c\<^sub>1 Q) \<and>\<^sub>p wp\<^sub>i (ncmp b) (wp R c\<^sub>2 Q))" |
+    "wp R (While b I c) Q = 
+      (stabilize R I \<and>\<^sub>p assert (I \<turnstile>\<^sub>p wp\<^sub>i (cmp b) (wp R c (stabilize R I)) \<and>\<^sub>p wp\<^sub>i (ncmp b) Q))" |
+    "wp R (DoWhile I c b) Q = 
+      (stabilize R I \<and>\<^sub>p assert (I \<turnstile>\<^sub>p wp R c (wp\<^sub>i (cmp b) (stabilize R I) \<and>\<^sub>p wp\<^sub>i (ncmp b) Q)))"
+
+text \<open>Convert a predicate transformer into a relational predicate transformer\<close>
+definition wp\<^sub>r :: "('v,'r,'a) trans \<Rightarrow> ('v,'r,'a) rtrans"
+  where "wp\<^sub>r f G \<equiv> \<lambda>(m,m'). f (\<lambda>m'. G (m,m')) m'"
+declare wp\<^sub>r_def [wp_defs]
+
+text \<open>Conditions under which a relational predicate is reflexive\<close>
+definition refl :: "('v,'r,'a) trel \<Rightarrow> ('v,'r,'a) pred"
+  where "refl G \<equiv> \<lambda>m. G (m,m)"
+declare refl_def [wp_defs]
+
+subsection \<open>Guarantee Checks\<close>
+
+text \<open>Convert a predicate transformer into a guarantee check\<close>
+abbreviation guar
+  where "guar f G \<equiv> refl (wp\<^sub>r f G)"
+
+text \<open>Ensure all global operations in a thread conform to its guarantee\<close>
 fun guar\<^sub>c
   where 
-    "guar\<^sub>c (Load v r\<^sub>a r a) G = 
-      (\<forall>m. v m \<longrightarrow> G (glb m,glb (m\<lparr>tstate.more := a (m(r :=\<^sub>r st m (rg m r\<^sub>a)))\<rparr>)))" |
-    "guar\<^sub>c (Store v r\<^sub>a r a) G = 
-      (\<forall>m. v m \<longrightarrow> G (glb m,glb (aux_upd a (m(rg m r\<^sub>a :=\<^sub>s rg m r)))))" |
-    "guar\<^sub>c (CAS v r\<^sub>a r\<^sub>1 r\<^sub>2 r T F a) G = 
-      ((\<forall>m. v m \<and> st m (rg m r\<^sub>a) = rg m r\<^sub>1 \<longrightarrow> G (glb m,glb (aux_upd a (m(rg m r\<^sub>a :=\<^sub>s rg m r\<^sub>2, r :=\<^sub>r T))))) \<and>
-      (\<forall>m. v m \<and> st m (rg m r\<^sub>a) \<noteq> rg m r\<^sub>1 \<longrightarrow> G (glb m,glb (aux_upd a (m(r :=\<^sub>r F))))))" |
+    "guar\<^sub>c (Load v r\<^sub>a r a) G = (v \<turnstile>\<^sub>p guar (wp_Load r\<^sub>a r a) (step G))" |
+    "guar\<^sub>c (Store v r\<^sub>a r a) G = (v \<turnstile>\<^sub>p guar (wp_Store r\<^sub>a r a) (step G))" |
+    "guar\<^sub>c (CAS v r\<^sub>a r\<^sub>1 r\<^sub>2 r T F a) G = (v \<turnstile>\<^sub>p guar (wp_CAS r\<^sub>a r\<^sub>1 r\<^sub>2 r T F a) (step G))" |
     "guar\<^sub>c (Seq c\<^sub>1 c\<^sub>2) G = (guar\<^sub>c c\<^sub>1 G \<and> guar\<^sub>c c\<^sub>2 G)" |
-    "guar\<^sub>c (If e\<^sub>1 f e\<^sub>2 c\<^sub>1 c\<^sub>2) G = (guar\<^sub>c c\<^sub>1 G \<and> guar\<^sub>c c\<^sub>2 G)" |
-    "guar\<^sub>c (While e\<^sub>1 f e\<^sub>2 I c) G = (guar\<^sub>c c G)" |
-    "guar\<^sub>c (DoWhile I c e\<^sub>1 f e\<^sub>2) G = (guar\<^sub>c c G)" |
+    "guar\<^sub>c (If b c\<^sub>1 c\<^sub>2) G = (guar\<^sub>c c\<^sub>1 G \<and> guar\<^sub>c c\<^sub>2 G)" |
+    "guar\<^sub>c (While b I c) G = (guar\<^sub>c c G)" |
+    "guar\<^sub>c (DoWhile I c b) G = (guar\<^sub>c c G)" |
     "guar\<^sub>c _ _ = True"
 
-section \<open>Soundness\<close>
+section \<open>Locale Interpretation\<close>
 
-text \<open>Convert the While language into the com language expected by the underlying logic\<close> 
-fun lift\<^sub>c :: "('v,'r,'a) lang \<Rightarrow> (('v,'r,'a) inst, ('v,'r,'a) tstate_scheme) com"
+text \<open>Convert the ARMv8 language into the abstract language expected by the underlying logic\<close> 
+fun lift\<^sub>c :: "('v,'r,'a) com_armv8 \<Rightarrow> (('v,'r,'a) auxop, ('v,'r,'a) tstate) com"
   where
     "lift\<^sub>c Skip = com.Nil" |
     "lift\<^sub>c Fence = Basic (\<lfloor>fence\<rfloor>)" |
     "lift\<^sub>c (Op r e) = Basic (\<lfloor>op r e\<rfloor>)" |
-    "lift\<^sub>c (Load c r\<^sub>a r a) = 
-      \<Sqinter> {[
-        \<lfloor>eq r\<^sub>a v\<^sub>a\<rfloor>, \<lfloor>(\<lambda>m. rg m r\<^sub>a = v\<^sub>a) \<and>\<^sub>p c,load v\<^sub>a (Val v) (\<lambda>m. a (m(r :=\<^sub>r v)))\<rfloor>, \<lfloor>op r (Glb v v\<^sub>a)\<rfloor>] 
-          |v v\<^sub>a. True}" |
-    "lift\<^sub>c (Store c r\<^sub>a r a) = \<Sqinter> {[\<lfloor>eq r\<^sub>a v\<^sub>a\<rfloor>, \<lfloor>(\<lambda>m. rg m r\<^sub>a = v\<^sub>a) \<and>\<^sub>p c,store v\<^sub>a (Reg r) a\<rfloor>] |v\<^sub>a. True}" |
+    "lift\<^sub>c (Load c r\<^sub>a r a) = \<Sqinter> {[
+      \<lfloor>eq ( r\<^sub>a) (Val v\<^sub>a)\<rfloor>, 
+      \<lfloor>(\<lambda>m. ev (rg m) r\<^sub>a = v\<^sub>a) \<and>\<^sub>p c,load v\<^sub>a (Val v), (\<lambda>m. a (m(r :=\<^sub>r v)))\<rfloor>, 
+      \<lfloor>op r (Glb v v\<^sub>a)\<rfloor>] |v v\<^sub>a. True}" |
+    "lift\<^sub>c (Store c r\<^sub>a r a) = \<Sqinter> {[
+      \<lfloor>eq ( r\<^sub>a) (Val v\<^sub>a)\<rfloor>, 
+      \<lfloor>(\<lambda>m. ev (rg m) r\<^sub>a = v\<^sub>a) \<and>\<^sub>p c,store v\<^sub>a (Reg r), a\<rfloor>] |v\<^sub>a. True}" |
     "lift\<^sub>c (CAS c r\<^sub>a r\<^sub>1 r\<^sub>2 r T F a) = (Choice
-      (\<Sqinter> {[\<lfloor>eq r\<^sub>a v\<^sub>a\<rfloor>, \<lfloor>(\<lambda>m. rg m r\<^sub>a = v\<^sub>a) \<and>\<^sub>p c,cas\<^sub>T v\<^sub>a (Reg r\<^sub>1) (Reg r\<^sub>2) (\<lambda>m. a (m(r :=\<^sub>r T)))\<rfloor>, \<lfloor>op r (Glb T v\<^sub>a)\<rfloor>] |v\<^sub>a. True})
-      (\<Sqinter> {[\<lfloor>eq r\<^sub>a v\<^sub>a\<rfloor>, \<lfloor>(\<lambda>m. rg m r\<^sub>a = v\<^sub>a) \<and>\<^sub>p c,cas\<^sub>F v\<^sub>a (Reg r\<^sub>1) (Reg r\<^sub>2) (\<lambda>m. a (m(r :=\<^sub>r F)))\<rfloor>, \<lfloor>op r (Glb F v\<^sub>a)\<rfloor>] |v\<^sub>a. True}))" |
+      (\<Sqinter> {[
+        \<lfloor>eq (Reg r\<^sub>a) (Val v\<^sub>a)\<rfloor>, 
+        \<lfloor>(\<lambda>m. rg m r\<^sub>a = v\<^sub>a) \<and>\<^sub>p c,cas\<^sub>T v\<^sub>a (Reg r\<^sub>1) (Reg r\<^sub>2),(\<lambda>m. a (m(r :=\<^sub>r T)))\<rfloor>, 
+        \<lfloor>op r (Glb T v\<^sub>a)\<rfloor>] |v\<^sub>a. True})
+      (\<Sqinter> {[
+        \<lfloor>eq (Reg r\<^sub>a) (Val v\<^sub>a)\<rfloor>, 
+        \<lfloor>(\<lambda>m. rg m r\<^sub>a = v\<^sub>a) \<and>\<^sub>p c,cas\<^sub>F v\<^sub>a (Reg r\<^sub>1) (Reg r\<^sub>2),(\<lambda>m. a (m(r :=\<^sub>r F)))\<rfloor>, 
+        \<lfloor>op r (Glb F v\<^sub>a)\<rfloor>] |v\<^sub>a. True}))" |
     "lift\<^sub>c (Seq c\<^sub>1 c\<^sub>2) = (lift\<^sub>c c\<^sub>1 ;; lift\<^sub>c c\<^sub>2)" |
-    "lift\<^sub>c (If e\<^sub>1 f e\<^sub>2 c\<^sub>1 c\<^sub>2) = (Choice (com.Seq (Basic (\<lfloor>cmp e\<^sub>1 f e\<^sub>2\<rfloor>)) (lift\<^sub>c c\<^sub>1)) 
-                                    (com.Seq (Basic (\<lfloor>ncmp e\<^sub>1 f e\<^sub>2\<rfloor>)) (lift\<^sub>c c\<^sub>2)))" |
-    "lift\<^sub>c (While e\<^sub>1 f e\<^sub>2 I c) = (com.Seq ((com.Seq (Basic (\<lfloor>cmp e\<^sub>1 f e\<^sub>2\<rfloor>)) (lift\<^sub>c c))*) 
-                                      (Basic (\<lfloor>ncmp e\<^sub>1 f e\<^sub>2\<rfloor>)))" |
-    "lift\<^sub>c (DoWhile I c e\<^sub>1 f e\<^sub>2) = (com.Seq ((com.Seq (lift\<^sub>c c) (Basic (\<lfloor>cmp e\<^sub>1 f e\<^sub>2\<rfloor>)))*) (com.Seq (lift\<^sub>c c) (Basic (\<lfloor>ncmp e\<^sub>1 f e\<^sub>2\<rfloor>))))" |
-    "lift\<^sub>c (Test p) = Basic (nop, UNIV, {(m,m'). m = m' \<and> p m})" |
-    "lift\<^sub>c (Assert p) = Basic (nop, Collect p, Id)"
+    "lift\<^sub>c (If b c\<^sub>1 c\<^sub>2) = (Choice 
+      (com.Seq (Basic (\<lfloor>cmp b\<rfloor>)) (lift\<^sub>c c\<^sub>1)) 
+      (com.Seq (Basic (\<lfloor>ncmp b\<rfloor>)) (lift\<^sub>c c\<^sub>2)))" |
+    "lift\<^sub>c (While b I c) = (com.Seq 
+      ((com.Seq (Basic (\<lfloor>cmp b\<rfloor>)) (lift\<^sub>c c))*) (Basic (\<lfloor>ncmp b\<rfloor>)))" |
+    "lift\<^sub>c (DoWhile I c b) = (com.Seq 
+      ((com.Seq (lift\<^sub>c c) (Basic (\<lfloor>cmp b\<rfloor>)))*) (com.Seq (lift\<^sub>c c) (Basic (\<lfloor>ncmp b\<rfloor>))))" |
+    "lift\<^sub>c (Test p) = Basic ((nop,tstate_rec.more), UNIV, {(m,m'). m = m' \<and> p m})" |
+    "lift\<^sub>c (Assert p) = Basic ((nop,tstate_rec.more), Collect p, Id)"
 
-subsection \<open>Interpretation of General Logic\<close>
-
-interpretation rules fwd\<^sub>s re\<^sub>i
+interpretation rules fwd\<^sub>s re\<^sub>a
   by (unfold_locales) (auto simp: pred_defs)
 
 abbreviation rules_abv ("_,_ \<turnstile> _ {_} _" [20,0,0,0,20] 20)
   where "rules_abv \<equiv> rules"
 
-abbreviation lifted_abv ("_,_ \<turnstile>\<^sub>s _ {_} _" [20,0,0,0,20] 20)
-  where "lifted_abv R G P c Q \<equiv> step\<^sub>R R,step G \<turnstile> Collect P {lift\<^sub>c c} Collect Q"
+abbreviation lifted_abv ("_,_,_ \<turnstile>\<^sub>s _ {_} _" [20,0,0,0,0,20] 20)
+  where "lifted_abv R G I P c Q \<equiv> \<langle>step\<^sub>t (inv I \<and>\<^sub>p R)\<rangle>,\<langle>step (inv I \<and>\<^sub>p G)\<rangle> \<turnstile> \<langle>all\<^sub>t I \<and>\<^sub>p P\<rangle> {lift\<^sub>c c} \<langle>all\<^sub>t I \<and>\<^sub>p Q\<rangle>"
 
-abbreviation validity_abv  ("\<Turnstile> _ SAT [_, _, _, _]" [60,0,0,0,0] 45) 
-  where "validity_abv c P R G Q \<equiv> validity (lift\<^sub>c c) (Collect P) (step\<^sub>R R) (step G) (Collect Q)"
+abbreviation validity_abv  ("\<Turnstile> _ SAT [_, _, _, _, _]" [60,0,0,0,0] 45) 
+  where "validity_abv c P R G Q I \<equiv> validity (lift\<^sub>c c) \<langle>all\<^sub>t I \<and>\<^sub>p P\<rangle> \<langle>step\<^sub>t (inv I \<and>\<^sub>p R)\<rangle> \<langle>step (inv I \<and>\<^sub>p G)\<rangle> \<langle>all\<^sub>t I \<and>\<^sub>p Q\<rangle>"
 
-text \<open>An ordering property on contexts\<close>
-definition context_order 
-  ("_,_ \<turnstile>\<^sub>w _ \<ge> _" [100,0,0,100] 60)
-  where "context_order R G P Q \<equiv> wellformed R G Q \<longrightarrow> ((P \<turnstile>\<^sub>p Q) \<and> wellformed R G P)"
-
-text \<open>The validity property we intend to show, abstracts over the preservation of wellformedness\<close>
-definition valid 
-  ("_,_ \<turnstile>\<^sub>w _ {_} _" [100,0,0,100] 60)
-  where "valid R G P c Q \<equiv> (guar\<^sub>c c G \<and> wellformed R G Q) \<longrightarrow> ((R,G \<turnstile>\<^sub>s P {c} Q) \<and> wellformed R G P)"
-
-subsection \<open>Instruction Soundness\<close>
-
-lemma [simp]:
-  "glb (m\<lparr>rg := e\<rparr>) = glb m"
-  unfolding glb_def by auto
-
-lemma [intro]:
-  "reflexive G \<Longrightarrow> G (m,m)"
-  by (auto simp: reflexive_def)
-
-lemma [intro!]:
-  "stable (step\<^sub>R R) (Collect Q) \<Longrightarrow> stable (step\<^sub>R R) {m. Q (m\<lparr>rg := f (rg m)\<rparr>)}"
-  by (auto simp add: wellformed_def stable_def step\<^sub>R_def)
-
-lemma [intro!]:
-  "stable (step\<^sub>R R) (Collect Q) \<Longrightarrow> stable (step\<^sub>R R) {m. f (rg m) \<longrightarrow> Q m}"
-  by (auto simp add: wellformed_def stable_def step\<^sub>R_def)
-
-fun stab\<^sub>i
-  where
-    "stab\<^sub>i R (load _ _ _) Q = stabilize R Q" |
-    "stab\<^sub>i R (store _ _ _) Q = stabilize R Q" |
-    "stab\<^sub>i R (cas\<^sub>T _ _ _ _) Q = stabilize R Q" |
-    "stab\<^sub>i R (cas\<^sub>F _ _ _ _) Q = stabilize R Q" |
-    "stab\<^sub>i _ _ Q = Q"
-
-lemma test[intro!]:
-  "wellformed R G Q \<Longrightarrow> wellformed R G (stab\<^sub>i R a (wp\<^sub>i a Q))"
-  by (cases a) (auto simp add: wellformed_def rg_upd_def)
-  
-lemma atomic_wp\<^sub>i:
-  assumes "wellformed R G Q" "c \<turnstile>\<^sub>p guar\<^sub>i a G"
-  shows "step\<^sub>R R,step G \<turnstile>\<^sub>A Collect (stabilize R (c \<and>\<^sub>p wp\<^sub>i a Q)) {\<lfloor>c, a\<rfloor>} Collect Q"
-  using assms by (cases a) (auto simp: atomic_rule_def guar_def wp_def rg_upd_def 
-                                       wellformed_def step_def aux_upd_def pred_defs 
-                                 elim!: stabilizeE)
-
-lemma atomic_wp\<^sub>i':
-  assumes "wellformed R G Q" "(\<lambda>m. True) \<turnstile>\<^sub>p guar\<^sub>i a G"
-  shows "step\<^sub>R R,step G \<turnstile>\<^sub>A Collect (stab\<^sub>i R a (wp\<^sub>i a Q)) {\<lfloor>a\<rfloor>} Collect Q"
-  using assms by (cases a) (auto simp: atomic_rule_def guar_def wp_def rg_upd_def 
-                                       wellformed_def step_def aux_upd_def pred_defs 
-                                 elim!: stabilizeE)
-
-lemma atomic_wp\<^sub>i_rw:
-  assumes "wellformed R G Q" "c \<turnstile>\<^sub>p guar\<^sub>i a G" "stable (step\<^sub>R R) (Collect P)" "P \<turnstile>\<^sub>p c \<and>\<^sub>p wp\<^sub>i a Q"
-  shows "step\<^sub>R R,step G \<turnstile>\<^sub>A Collect P {\<lfloor>c, a\<rfloor>} Collect Q"
-  using assms by (cases a) (auto simp: atomic_rule_def guar_def wp_def rg_upd_def 
-                                       wellformed_def step_def aux_upd_def pred_defs 
-                                 elim!: stabilizeE)
-
-lemma atomic_wp\<^sub>i_rw':
-  assumes "wellformed R G Q" "(\<lambda>m. True) \<turnstile>\<^sub>p guar\<^sub>i a G" "stable (step\<^sub>R R) (Collect P)" "P \<turnstile>\<^sub>p wp\<^sub>i a Q"
-  shows "step\<^sub>R R,step G \<turnstile>\<^sub>A Collect P {\<lfloor>a\<rfloor>} Collect Q"
-  using assms by (cases a) (auto simp: atomic_rule_def guar_def wp_def rg_upd_def 
-                                       wellformed_def step_def aux_upd_def pred_defs 
-                                 elim!: stabilizeE)
-
-(*
-lemma atomic_op [intro]:
-  "wellformed R G Q \<Longrightarrow> step\<^sub>R R,step G \<turnstile>\<^sub>A Collect (wp\<^sub>i R (op r e) Q) {\<lfloor>op r e\<rfloor>} Collect Q"
-  by (auto simp: atomic_rule_def guar_def wp_def rg_upd_def wellformed_def step_def)
-
-lemma atomic_cmp [intro]:
-  "wellformed R G Q \<Longrightarrow> step\<^sub>R R,step G \<turnstile>\<^sub>A Collect (wp\<^sub>i R (cmp e\<^sub>1 f e\<^sub>2) Q) {\<lfloor>cmp e\<^sub>1 f e\<^sub>2\<rfloor>} Collect Q"
-  by (auto simp: atomic_rule_def guar_def wp_def wellformed_def step_def)
-
-lemma atomic_load [intro]:
-  assumes "wellformed R G Q" "guar\<^sub>c (Load c r\<^sub>a r a) G"
-  shows "step\<^sub>R R,step G \<turnstile>\<^sub>A Collect (stabilize R (c \<and>\<^sub>p wp\<^sub>i (load v\<^sub>a e a) Q)) {\<lfloor>c, load v\<^sub>a e a\<rfloor>} Collect Q"
-  using assms by (auto simp: atomic_rule_def wp_def pred_defs guar_def step_def wellformed_def elim!: stabilizeE)
-*)
-
-lemma nil [intro]:
-  assumes "wellformed R G Q"
-  shows "step\<^sub>R R,step G \<turnstile> Collect Q {Nil} Collect Q" 
-  using assms by (auto simp: wellformed_def)
-
-lemma [simp]:
-  "rg (set_glb m g) r\<^sub>a = rg m r\<^sub>a"
-  by (auto simp: set_glb_def)
-
-lemma [simp]:
-  "set_glb (set_glb m g) g' = set_glb m g'"
-  by (auto simp: set_glb_def)
-
-lemma [simp]:
-  "set_glb (m\<lparr>tstate.more := a\<rparr>) g = set_glb m g"
-    by (auto simp: set_glb_def)
-
-lemma [simp]:
-  "st (set_glb m g) = st g"
-  by (auto simp: set_glb_def)
-
-lemma [simp]:
-  "m(r :=\<^sub>r e)\<lparr>tstate.more := a\<rparr> = (m\<lparr>tstate.more := a\<rparr>)(r :=\<^sub>r e)"
-  by (auto simp: rg_upd_def)
-
-lemma ord_rotate:
-  "R,G \<turnstile> Q {c\<^sub>2} M \<Longrightarrow> R,G \<turnstile> P {c\<^sub>1} Q \<Longrightarrow> R,G \<turnstile> P {c\<^sub>1 \<cdot> c\<^sub>2} M"
-  by auto
-
-lemma load_sound:
-  assumes "wellformed R G Q" "guar\<^sub>c (Load c r\<^sub>a r a) G"
-  shows "R,G \<turnstile>\<^sub>s wp R G (Load c r\<^sub>a r a) Q {Load c r\<^sub>a r a} Q"
-  using assms
-  apply (clarsimp simp del: beh\<^sub>i.simps)
-  apply (intro rules.seqset)
-  apply (clarsimp simp del: beh\<^sub>i.simps)
-  apply (intro ord_rotate rules.basic)
-  apply (rule nil, simp)
-  apply (rule atomic_wp\<^sub>i')
-  apply (auto simp add: pred_defs)[2]
-  apply (rule atomic_wp\<^sub>i)
-  apply blast
-  apply (auto simp add: pred_defs aux_upd_def rg_upd_def)[1]
-  apply (rule atomic_wp\<^sub>i_rw')
-  apply auto
-  apply (auto simp: stabilize_def aux_upd_def pred_defs)
-  done
-
-lemma store_sound:
-  assumes "wellformed R G Q" "guar\<^sub>c (Store c r\<^sub>a r a) G"
-  shows "R,G \<turnstile>\<^sub>s wp R G (Store c r\<^sub>a r a) Q {Store c r\<^sub>a r a} Q"
-  using assms
-  apply (clarsimp simp del: beh\<^sub>i.simps)
-  apply (intro rules.seqset)
-  apply (clarsimp simp del: beh\<^sub>i.simps)
-  apply (intro ord_rotate rules.basic)
-  apply (rule nil, simp)
-  apply (rule atomic_wp\<^sub>i)
-  apply (auto simp add: pred_defs aux_upd_def rg_upd_def)[2]
-  apply (rule atomic_wp\<^sub>i_rw')
-  apply auto
-  apply (auto simp: stabilize_def aux_upd_def pred_defs)
-  done
-
-lemma [simp]:
-  "glb (m(r :=\<^sub>r T)) = glb m"
-  by (auto simp: glb_def rg_upd_def)
-
-lemma cas_sound:
-  assumes "wellformed R G Q" "guar\<^sub>c (CAS c r\<^sub>a r\<^sub>1 r\<^sub>2 r T F a) G"
-  shows "R,G \<turnstile>\<^sub>s wp R G (CAS c r\<^sub>a r\<^sub>1 r\<^sub>2 r T F a) Q {CAS c r\<^sub>a r\<^sub>1 r\<^sub>2 r T F a} Q"
-  using assms
-  apply (clarsimp simp del: beh\<^sub>i.simps)
-  apply (intro rules.choice rules.seqset)
-  apply (clarsimp simp del: beh\<^sub>i.simps)
-  apply (intro ord_rotate rules.basic)
-  apply (rule nil, simp)
-  apply (rule atomic_wp\<^sub>i'; auto simp add: pred_defs)
-  apply (rule atomic_wp\<^sub>i)
-  apply blast
-  apply (auto simp add: pred_defs aux_upd_def)[1]
-  apply (rule atomic_wp\<^sub>i_rw')
-  apply auto[3]
-  apply (auto simp: stabilize_def aux_upd_def pred_defs)[1]
-  apply (clarsimp simp del: beh\<^sub>i.simps)
-  apply (intro ord_rotate rules.basic)
-  apply (rule nil, simp)
-  apply (rule atomic_wp\<^sub>i'; auto simp add: pred_defs)
-  apply (rule atomic_wp\<^sub>i)
-  apply blast
-  apply (auto simp add: pred_defs aux_upd_def)[1]
-  apply (rule atomic_wp\<^sub>i_rw')
-  apply auto[3]  
-  apply (auto simp: stabilize_def aux_upd_def pred_defs)[1]
-  done
-
-lemma op_sound:
-  assumes "wellformed R G Q"
-  shows "R,G \<turnstile>\<^sub>s wp R G (Op r e) Q {Op r e} Q"
-  using assms
-  apply (clarsimp simp del: wp.simps beh\<^sub>i.simps)
-  apply (rule rules.basic)
-  apply (rule atomic_wp\<^sub>i_rw')
-  apply (auto simp: pred_defs)
-  by (auto simp: wellformed_def rg_upd_def)
-
-lemma fence_sound:
-  assumes "wellformed R G Q"
-  shows "R,G \<turnstile>\<^sub>s wp R G (Fence) Q {Fence} Q"
-  apply (clarsimp, rule rules.basic, simp add: atomic_rule_def, intro conjI)
-  using assms
-  by (auto simp: wp_def pred_defs step_def guar_def wellformed_def reflexive_def)
-
-lemma test_sound:
-  assumes "wellformed R G Q"
-  shows "R,G \<turnstile>\<^sub>s wp R G (Test p) Q {Test p} Q"
-  apply (clarsimp, rule rules.basic, simp add: atomic_rule_def, intro conjI)
-  using assms
-  apply (auto simp: wp_def pred_defs elim!: stabilizeE)
-  by (auto simp: step_def guar_def wellformed_def reflexive_def)
-
-lemma assert_sound:
-  assumes "wellformed R G Q"
-  shows "R,G \<turnstile>\<^sub>s wp R G (Assert p) Q {Assert p} Q"
-  apply (clarsimp, rule rules.basic, simp add: atomic_rule_def, intro conjI)
-  using assms
-  apply (auto simp: wp_def pred_defs elim!: stabilizeE)[1]
-  using assms
-  apply (auto simp: step_def guar_def wellformed_def reflexive_def)
-  using assms by blast
-
-subsection \<open>Base Introduction Rules\<close>
-
-text \<open>Reflexive Ordering\<close>
-lemma ord_refl [intro]:
-  "R,G \<turnstile>\<^sub>w P \<ge> P"
-  unfolding context_order_def by (auto simp: pred_defs)
-
-text \<open>Assert Ordering\<close>
-lemma ord_assert:
-  "R,G \<turnstile>\<^sub>w P \<and>\<^sub>p assert A \<ge> P"
-  by (cases A) (auto simp: context_order_def pred_defs intro: wf_false) 
-
-text \<open>Stabilize Ordering\<close>
-lemma ord_stabilize:
-  assumes "P \<turnstile>\<^sub>p Q" 
-  shows "R,G \<turnstile>\<^sub>w stabilize R P \<ge> Q"
-  using assms stabilizeE unfolding context_order_def entail_def
-  by blast
-
-text \<open>Skip Rule\<close>
-lemma skip_wp:
-  "R,G \<turnstile>\<^sub>w Q {Skip} Q"
-  by (auto simp: context_order_def valid_def wellformed_def)
-
-text \<open>Sequential Rule\<close>
-lemma seq_wp:
-  "R,G \<turnstile>\<^sub>w P {c\<^sub>1} Q \<Longrightarrow> R,G \<turnstile>\<^sub>w M {c\<^sub>2} P \<Longrightarrow> R,G \<turnstile>\<^sub>w M {Seq c\<^sub>2 c\<^sub>1} Q"
-  unfolding valid_def by auto
-
-text \<open>Stabilization preserves entailment\<close>
-lemma stabilize_entail [intro]:
-  assumes "P \<turnstile>\<^sub>p Q"
-  shows "stabilize R P \<turnstile>\<^sub>p stabilize R Q"
-  using assms by (clarsimp simp add: entail_def stabilize_def)
-
-lemma stabilize_entail' [intro]:
-  assumes "wellformed R G Z"
-  assumes "P \<turnstile>\<^sub>p Q"
-  shows "stabilize R P \<turnstile>\<^sub>p Q"
-  using assms
-  by (clarsimp simp add: entail_def stabilize_def wellformed_def stable_def step\<^sub>R_def reflexive_def)
-
-lemma cmp_sound:
-  assumes "wellformed R G Q"
-  assumes "P \<turnstile>\<^sub>p wp\<^sub>i (cmp e\<^sub>1 f e\<^sub>2) Q"
-  shows "step\<^sub>R R,step G \<turnstile> Collect P {Basic (\<lfloor>cmp e\<^sub>1 f e\<^sub>2\<rfloor>)} Collect Q"
-  apply (rule rules.conseq[of "step\<^sub>R R" "step G" "Collect (wp\<^sub>i (cmp e\<^sub>1 f e\<^sub>2) Q)" _ "Collect Q"])
-  apply (rule rules.basic)
-  unfolding atomic_rule_def
-  apply (intro conjI)
-  apply (clarsimp simp: wp_def)
-  using assms apply (clarsimp simp: guar_def wellformed_def reflexive_def step_def)
-  using assms apply (auto simp: wellformed_def step\<^sub>R_def stable_def)[2]
-  using assms(2) apply (clarsimp simp: pred_defs)[1]
-  by auto
-  
-text \<open>If Rule\<close>
-lemma ifWP:
-  assumes "R,G \<turnstile>\<^sub>w P\<^sub>1 {c\<^sub>1} Q"
-  assumes "R,G \<turnstile>\<^sub>w P\<^sub>2 {c\<^sub>2} Q"
-  shows "R,G \<turnstile>\<^sub>w (wp\<^sub>i (cmp e\<^sub>1 f e\<^sub>2) P\<^sub>1 \<and>\<^sub>p wp\<^sub>i (ncmp e\<^sub>1 f e\<^sub>2) P\<^sub>2) {If e\<^sub>1 f e\<^sub>2 c\<^sub>1 c\<^sub>2} Q"
-  using assms
-  unfolding valid_def
-  apply (clarsimp simp del: beh\<^sub>i.simps)
-  apply (intro impI conjI rules.choice rules.seq stabilize_wellformed; assumption?)
-  apply (rule cmp_sound; simp)
-  apply (simp add: pred_defs)
-  apply (rule cmp_sound; simp)
-  apply (simp add: pred_defs)
-  unfolding wellformed_def
-  apply simp
-  by (auto simp: stable_def step\<^sub>R_def pred_defs)
-
-text \<open>While Rule\<close>
-lemma whileWP:
-  assumes "I \<turnstile>\<^sub>p wp\<^sub>i (cmp e\<^sub>1 f e\<^sub>2) P \<and>\<^sub>p wp\<^sub>i (ncmp e\<^sub>1 f e\<^sub>2) Q"
-  assumes "R,G \<turnstile>\<^sub>w P {c} stabilize R I" (is "R,G \<turnstile>\<^sub>w P {c} ?I")
-  shows "R,G \<turnstile>\<^sub>w ?I {While e\<^sub>1 f e\<^sub>2 I c} Q"
-  unfolding valid_def lift\<^sub>c.simps
-proof (intro impI conjI rules.choice rules.seq stabilize_wellformed; assumption?)
-  assume "guar\<^sub>c (While e\<^sub>1 f e\<^sub>2 I c) G \<and> wellformed R G Q"
-  thus "step\<^sub>R R,step G \<turnstile> (Collect ?I) {Basic (\<lfloor>ncmp e\<^sub>1 f e\<^sub>2\<rfloor>)} Collect Q"
-    using assms(1) by (intro cmp_sound; simp; intro stabilize_entail'; simp add: pred_defs)
-next
-  assume "guar\<^sub>c (While e\<^sub>1 f e\<^sub>2 I c) G \<and> wellformed R G Q"
-  hence "guar\<^sub>c c G" "wellformed R G ?I" by auto
-  thus "step\<^sub>R R,step G \<turnstile> Collect ?I {(Basic (\<lfloor>cmp e\<^sub>1 f e\<^sub>2\<rfloor>) ;; lift\<^sub>c c)*} Collect ?I"
-    using assms
-    apply (intro rules.loop rules.seq stabilize_stable; unfold valid_def)
-    apply blast
-    defer 1
-    apply blast
-    apply (intro cmp_sound; simp; intro stabilize_entail'; simp add: pred_defs)
-    done
-qed auto
-
-lemma doWhileWP:
-  assumes "R,G \<turnstile>\<^sub>w stabilize R I {c} (wp\<^sub>i (cmp e\<^sub>1 f e\<^sub>2) (stabilize R I) \<and>\<^sub>p wp\<^sub>i (ncmp e\<^sub>1 f e\<^sub>2) Q)" (is "R,G \<turnstile>\<^sub>w ?I {c} ?Q")
-  shows "R,G \<turnstile>\<^sub>w stabilize R I {DoWhile I c e\<^sub>1 f e\<^sub>2} Q"
-  unfolding valid_def lift\<^sub>c.simps
-proof (intro impI conjI rules.choice rules.seq stabilize_wellformed; assumption?)
-  assume "guar\<^sub>c (DoWhile I c e\<^sub>1 f e\<^sub>2) G \<and> wellformed R G Q"
-  thus "step\<^sub>R R,step G \<turnstile> Collect ?Q {Basic (\<lfloor>ncmp e\<^sub>1 f e\<^sub>2\<rfloor>)} Collect Q"
-    by (intro cmp_sound; simp add: pred_defs)
-next
-  assume "guar\<^sub>c (DoWhile I c e\<^sub>1 f e\<^sub>2) G \<and> wellformed R G Q"
-  hence "guar\<^sub>c c G \<and> wellformed R G ?Q" sorry
-  thus "step\<^sub>R R,step G \<turnstile> Collect ?I {lift\<^sub>c c} Collect ?Q"
-    using assms(1) unfolding valid_def by simp 
-next
-  assume wf: "guar\<^sub>c (DoWhile I c e\<^sub>1 f e\<^sub>2) G \<and> wellformed R G Q"
-  hence "wellformed R G ?I \<and> wellformed R G ?Q \<and> guar\<^sub>c c G" sorry
-  thus "step\<^sub>R R,step G \<turnstile> Collect ?I {(lift\<^sub>c c ;; Basic (\<lfloor>cmp e\<^sub>1 f e\<^sub>2\<rfloor>))*} Collect ?I"
-    using assms
-    apply (intro rules.loop rules.seq stabilize_stable; unfold valid_def)
-    apply blast
-    apply blast
-    by (intro cmp_sound; simp add: pred_defs)
-qed auto
-
+text \<open>The language is always thread-local\<close>
 lemma local_lift [intro]:
   "local (lift\<^sub>c c)"
   by (induct c) auto
 
-lemma guar_all:
-  "wellformed R G Q \<Longrightarrow> guar\<^sub>c c G \<Longrightarrow> \<forall>\<beta>\<in>basics (lift\<^sub>c c). guar\<^sub>\<alpha> \<beta> (step G)"
-  sorry (*apply (induct c) 
-  apply (auto simp: guar_def step_def pred_defs wellformed_def reflexive_def)
-  apply (subgoal_tac "G (ab, ab(ba x2 := ba x3))")
-  apply (subgoal_tac "(ab(ba x2 := ba x3)) = (\<lambda>x. if x = ba x2 then rg (ab, ba) x3 else ld (ab,ba) x)")
-  apply simp
-  apply auto
-  apply (subgoal_tac " G (ab, ab(ba x2 := ba x4))")
-  apply (subgoal_tac "(ab(ba x2 := ba x4)) = (\<lambda>x. if x = ba x2 then rg (ab, ba) x4 else ld (ab,ba) x)")
-  apply simp
-  apply auto
-  done *)
+text \<open>Correctness of the guarantee check\<close>
+lemma com_guar:
+  "wellformed R G \<Longrightarrow> guar\<^sub>c c G \<Longrightarrow> \<forall>\<beta>\<in>basics (lift\<^sub>c c). guar\<^sub>\<alpha> \<beta> \<langle>step G\<rangle>"
+  by (induct c) (auto simp: guar_def step_def reflexive_def wp_defs pred_defs liftl_def liftg_def)
+
+text \<open>An ordering property on contexts\<close>
+definition context_order 
+  ("_,_ \<turnstile>\<^sub>w _ \<ge> _" [100,0,0,100] 60)
+  where "context_order R G P Q \<equiv> 
+    (stable\<^sub>t R Q \<and> wellformed R G) \<longrightarrow> ((P \<turnstile>\<^sub>p Q) \<and> stable\<^sub>t R P)"
+
+text \<open>The validity property we intend to show, abstracts over the preservation of wellformedness\<close>
+definition valid :: "('v,'a) grel \<Rightarrow> ('v,'a) grel \<Rightarrow> ('v,'a) gpred \<Rightarrow> ('v,'r,'a) pred \<Rightarrow> ('v,'r,'a) com_armv8 \<Rightarrow> ('v,'r,'a) pred \<Rightarrow> bool"
+  ("_,_,_ \<turnstile>\<^sub>w _ {_} _" [100,0,0,0,0,100] 60)
+  where "valid R G I P c Q \<equiv>  
+    (wellformed R G \<and> stable\<^sub>t R Q \<and> guar\<^sub>c c (inv I \<and>\<^sub>p G)) \<longrightarrow> (stable\<^sub>t R P \<and> (R,G,I \<turnstile>\<^sub>s P {c} Q))"
+
+section \<open>Soundness\<close>
+
+subsection \<open>Sub-operations\<close>
+
+lemma stable\<^sub>t_local_op [intro!]:
+  "stable\<^sub>t R Q \<Longrightarrow> stable\<^sub>t R (\<lambda>m. Q (m\<lparr>rg := f (rg m)\<rparr>))"
+  by (auto simp add: stable_def step\<^sub>t_def)
+
+lemma stable\<^sub>t_local_cmp [intro!]:
+  "stable\<^sub>t R Q \<Longrightarrow> stable\<^sub>t R (\<lambda>m. f (rg m) \<longrightarrow> Q m)"
+  by (auto simp add: stable_def step\<^sub>t_def)
+
+lemma stable\<^sub>t_local_assign [intro!]:
+  "stable\<^sub>t R Q \<Longrightarrow> stable\<^sub>t R (\<lambda>m. Q (m(r :=\<^sub>r f (rg m))))"
+  unfolding rg_upd_def by auto
+
+fun local_op
+  where
+    "local_op (load _ _) = False" |
+    "local_op (store _ _) = False" |
+    "local_op (cas\<^sub>T _ _ _) = False" |
+    "local_op (cas\<^sub>F _ _ _) = False" |
+    "local_op _ = True"
+
+lemma [intro]:
+  "(inv I) (m,m)"
+  by (auto simp: inv_def)
+
+lemma [intro!]:
+  "stable\<^sub>t R Q \<Longrightarrow> stable\<^sub>t ((\<lambda>(m, m'). I m \<longrightarrow> I m') \<and>\<^sub>p R) (\<lambda>m. I (glb m) \<and> Q m)"
+  by (auto simp: stable_def step\<^sub>t_def inv_def)
+
+lemma [intro!]:
+  "stable\<^sub>t R Q \<Longrightarrow> stable\<^sub>t (inv I \<and>\<^sub>p R) (all\<^sub>t I \<and>\<^sub>p Q)"
+  by (auto simp: stable_def step\<^sub>t_def inv_def all\<^sub>t_def)
+
+lemma [intro!]:
+  "reflexive G \<Longrightarrow> reflexive (inv I \<and>\<^sub>p G)"
+  by (auto simp: reflexive_def inv_def)
+
+text \<open>Basic Rule for global operations\<close>
+lemma basic_wp\<^sub>i_global:
+  assumes "P \<turnstile>\<^sub>p stabilize R (c \<and>\<^sub>p wp\<^sub>i \<alpha> (wp\<^sub>a a Q))" "wellformed R G" "stable\<^sub>t R Q" 
+  assumes "c \<turnstile>\<^sub>p guar (wp\<^sub>i \<alpha> o wp\<^sub>a a) (step (inv I \<and>\<^sub>p G))"
+  shows "\<langle>step\<^sub>t (inv I \<and>\<^sub>p R)\<rangle>,\<langle>step (inv I \<and>\<^sub>p G)\<rangle> \<turnstile> \<langle>all\<^sub>t I \<and>\<^sub>p P\<rangle> {Basic (\<lfloor>c, \<alpha>, a\<rfloor>)} \<langle>all\<^sub>t I \<and>\<^sub>p Q\<rangle>"
+proof -
+  have "\<langle>step\<^sub>t (inv I \<and>\<^sub>p R)\<rangle>,\<langle>step (inv I \<and>\<^sub>p G)\<rangle> \<turnstile>\<^sub>A \<langle>all\<^sub>t I \<and>\<^sub>p stabilize R (c \<and>\<^sub>p wp\<^sub>i \<alpha> (wp\<^sub>a a Q))\<rangle> {\<lfloor>c, \<alpha>, a\<rfloor>} \<langle>all\<^sub>t I \<and>\<^sub>p Q\<rangle>"
+    using assms by (cases \<alpha>) (auto simp: atomic_rule_def guar_def wp_def rg_upd_def 
+                                         step_def aux_upd_def pred_defs 
+                                         refl_def wp\<^sub>r_def o_def liftg_def all\<^sub>t_def inv_def
+                                   elim!: stabilizeE)
+  thus ?thesis using assms by (intro conseq[OF basic]) (auto simp: pred_defs)
+qed
+
+text \<open>Basic Rule for local operations\<close>
+lemma basic_wp\<^sub>i_local:
+  assumes "P \<turnstile>\<^sub>p wp\<^sub>i \<alpha> Q" "wellformed R G" "stable\<^sub>t R Q" "local_op \<alpha>" 
+  shows "\<langle>step\<^sub>t (inv I \<and>\<^sub>p R)\<rangle>,\<langle>step (inv I \<and>\<^sub>p G)\<rangle> \<turnstile> \<langle>all\<^sub>t I \<and>\<^sub>p P\<rangle> {Basic (\<lfloor>\<alpha>\<rfloor>)} \<langle>all\<^sub>t I \<and>\<^sub>p Q\<rangle>"
+proof -
+  have "\<langle>step\<^sub>t (inv I \<and>\<^sub>p R)\<rangle>,\<langle>step (inv I \<and>\<^sub>p G)\<rangle> \<turnstile>\<^sub>A  \<langle>all\<^sub>t I \<and>\<^sub>p wp\<^sub>i \<alpha> Q\<rangle> {\<lfloor>\<alpha>\<rfloor>} \<langle>all\<^sub>t I \<and>\<^sub>p Q\<rangle>"
+    using assms by (cases \<alpha>) (auto simp: atomic_rule_def guar_def wp_def rg_upd_def 
+                                         step_def aux_upd_def pred_defs liftl_def all\<^sub>t_def inv_def
+                                         elim!: stabilizeE)
+  thus ?thesis using assms by (intro conseq[OF basic]) (auto simp: pred_defs)
+qed
+
+text \<open>Automation to assist with Load/Store/CAS\<close>
+lemma stabilize_cmp:
+  "P \<turnstile>\<^sub>p wp\<^sub>i (cmp b) Q \<Longrightarrow> stabilize R P \<turnstile>\<^sub>p wp\<^sub>i (cmp b) (stabilize R Q)"
+  by (auto simp: pred_defs stabilize_def set_glb_def)
+
+method expand_seq =
+  (clarsimp, intro rules.choice rules.seqset; (clarsimp, intro rules.ord, (auto)[1]))
+
+method basic_wp\<^sub>i = 
+  ((rule basic_wp\<^sub>i_local | rule basic_wp\<^sub>i_global), 
+   (rule stabilize_cmp | fast); 
+   auto simp: wp_defs pred_defs step_def aux_upd_def)
+
+text \<open>A rule for cmp operations, used for If/While/DoWhile\<close>
+lemma cmp_sound [intro!]:
+  assumes "wellformed R G" "stable\<^sub>t R Q"
+  assumes "P \<turnstile>\<^sub>p wp\<^sub>i (cmp b) Q"
+  shows "\<langle>step\<^sub>t (inv I \<and>\<^sub>p R)\<rangle>,\<langle>step (inv I \<and>\<^sub>p G)\<rangle> \<turnstile> \<langle>all\<^sub>t I \<and>\<^sub>p P\<rangle> {Basic (\<lfloor>cmp b\<rfloor>)} \<langle>all\<^sub>t I \<and>\<^sub>p Q\<rangle>"
+  using assms by (intro basic_wp\<^sub>i_local) auto
+
+subsection \<open>State Ordering\<close>
+
+text \<open>Properties of the state ordering. Essentially entailment with preservation of stability\<close>
+
+text \<open>The ordering is reflexive\<close>
+lemma refl_ord:
+  "R,G \<turnstile>\<^sub>w P \<ge> P"
+  unfolding context_order_def by (auto simp: pred_defs)
+
+text \<open>It is possible to strengthen the RHS\<close>
+lemma assert_ord:
+  "R,G \<turnstile>\<^sub>w P \<and>\<^sub>p assert A \<ge> P"
+  by (cases A) (auto simp: context_order_def assert_def) 
+
+text \<open>Stabilize Ordering\<close>
+lemma stabilize_ord [intro]:
+  assumes "P \<turnstile>\<^sub>p Q" 
+  shows "R,G \<turnstile>\<^sub>w stabilize R P \<ge> Q"
+  using assms stabilizeE unfolding context_order_def 
+  by blast
+
+subsection \<open>Rules\<close>
+
+text \<open>If Rule\<close>
+lemma if_wp:
+  "R,G,I \<turnstile>\<^sub>w P\<^sub>1 {c\<^sub>1} Q \<Longrightarrow> R,G,I \<turnstile>\<^sub>w P\<^sub>2 {c\<^sub>2} Q \<Longrightarrow> R,G,I \<turnstile>\<^sub>w wp\<^sub>i (cmp b) P\<^sub>1 \<and>\<^sub>p wp\<^sub>i (ncmp b) P\<^sub>2 {If b c\<^sub>1 c\<^sub>2} Q"
+  unfolding valid_def by clarsimp (intro conjI rules.choice rules.seq, auto simp add: pred_defs)
+
+text \<open>While Rule\<close>
+lemma while_wp:
+  assumes "R,G,I \<turnstile>\<^sub>w P {c} stabilize R J" (is "R,G,I \<turnstile>\<^sub>w P {c} ?I")
+  assumes "J \<turnstile>\<^sub>p wp\<^sub>i (cmp b) P \<and>\<^sub>p wp\<^sub>i (ncmp b) Q"
+  shows "R,G,I \<turnstile>\<^sub>w ?I {While b J c} Q"
+  unfolding valid_def lift\<^sub>c.simps
+proof (intro impI conjI rules.choice rules.seq)
+  assume "wellformed R G \<and> stable\<^sub>t R Q \<and> guar\<^sub>c (While b J c) (inv I \<and>\<^sub>p G)"
+  thus "\<langle>step\<^sub>t (inv I \<and>\<^sub>p R)\<rangle>,\<langle>step (inv I \<and>\<^sub>p G)\<rangle> \<turnstile> \<langle>all\<^sub>t I \<and>\<^sub>p ?I\<rangle> {(Basic (\<lfloor>cmp b\<rfloor>) ;; lift\<^sub>c c)*} \<langle>all\<^sub>t I \<and>\<^sub>p ?I\<rangle>"
+    using assms 
+    apply (intro rules.loop rules.seq, unfold valid_def)
+    apply force
+    apply force
+    by (auto elim!: stabilizeE)
+qed (insert assms, auto simp add: pred_defs elim!: stabilizeE)
+
+text \<open>Do While Rule\<close>
+lemma do_wp:
+  assumes "R,G,I \<turnstile>\<^sub>w stabilize R J {c} (wp\<^sub>i (cmp b) (stabilize R J) \<and>\<^sub>p wp\<^sub>i (ncmp b) Q)" (is "R,G,I \<turnstile>\<^sub>w ?I {c} ?Q")
+  shows "R,G,I \<turnstile>\<^sub>w stabilize R J {DoWhile J c b} Q"
+  unfolding valid_def lift\<^sub>c.simps
+proof (intro impI conjI rules.choice rules.seq)
+  assume "wellformed R G \<and> stable\<^sub>t R Q \<and> guar\<^sub>c (DoWhile J c b) (inv I \<and>\<^sub>p G)"
+  thus "\<langle>step\<^sub>t (inv I \<and>\<^sub>p R)\<rangle>,\<langle>step (inv I \<and>\<^sub>p G)\<rangle> \<turnstile> \<langle>all\<^sub>t I \<and>\<^sub>p ?I\<rangle> {lift\<^sub>c c} \<langle>all\<^sub>t I \<and>\<^sub>p ?Q\<rangle>" 
+    using assms by (auto simp: valid_def) 
+next
+  assume "wellformed R G \<and> stable\<^sub>t R Q \<and> guar\<^sub>c (DoWhile J c b) (inv I \<and>\<^sub>p G)"
+  thus "\<langle>step\<^sub>t (inv I \<and>\<^sub>p R)\<rangle>,\<langle>step (inv I \<and>\<^sub>p G)\<rangle> \<turnstile> \<langle>all\<^sub>t I \<and>\<^sub>p ?I\<rangle> {(lift\<^sub>c c ;; Basic (\<lfloor>cmp b\<rfloor>))*} \<langle>all\<^sub>t I \<and>\<^sub>p ?I\<rangle>"
+    using assms 
+    apply (intro rules.loop seq_rot)
+    apply (auto simp: valid_def)[2]
+    by auto
+qed (insert assms, auto simp add: pred_defs)
 
 text \<open>False Rule\<close>
-lemma falseWP:
+lemma false_wp:
   assumes "P \<turnstile>\<^sub>p (\<lambda>m. False)"
-  shows "R,G \<turnstile>\<^sub>w P {c} Q"
+  shows "R,G,I \<turnstile>\<^sub>w P {c} Q"
   using assms unfolding valid_def
-  apply (intro conjI impI guar_all rules.conseq[OF falseI, where ?G="step G"])
-  by (auto simp: entail_def intro: wf_false)
+  by (intro conjI impI com_guar rules.conseq[OF falseI, where ?G="\<langle>step (inv I \<and>\<^sub>p G)\<rangle>"]) (auto simp: )
 
-text \<open>Precondition Rewrite Rule\<close>
-lemma rewriteWP:
-  "R,G \<turnstile>\<^sub>w P {c} Q \<Longrightarrow> R,G \<turnstile>\<^sub>w M \<ge> P \<Longrightarrow> R,G \<turnstile>\<^sub>w M {c} Q"
-proof (clarsimp simp add: valid_def context_order_def)
-  assume a: "M \<turnstile>\<^sub>p P"
-  assume "R,G \<turnstile>\<^sub>s P {c} Q "
-  thus "R,G \<turnstile>\<^sub>s M {c} Q" by (rule rules.conseq) (insert a, auto simp: entail_def)
-qed
+text \<open>Rewrite Rule\<close>
+lemma rewrite_wp:
+  "R,G,I \<turnstile>\<^sub>w P {c} Q \<Longrightarrow> R,G \<turnstile>\<^sub>w M \<ge> P \<Longrightarrow> R,G,I \<turnstile>\<^sub>w M {c} Q"
+  by (auto simp: valid_def context_order_def)
 
 text \<open>Assert Rule\<close>
-
-lemma assertWP:
-  assumes "A \<longrightarrow> R,G \<turnstile>\<^sub>w P {c} Q"
-  shows "R,G \<turnstile>\<^sub>w (P \<and>\<^sub>p assert A) {c} Q"
+lemma assert_wp:
+  assumes "A \<Longrightarrow> R,G,I \<turnstile>\<^sub>w P {c} Q"
+  shows "R,G,I \<turnstile>\<^sub>w (P \<and>\<^sub>p assert A) {c} Q"
 proof (cases A)
   case True
-  then show ?thesis using assms by (intro rewriteWP[OF _ ord_assert], simp)
+  then show ?thesis using assms by (intro rewrite_wp[OF _ assert_ord], simp)
 next
   case False
-  then show ?thesis by (intro falseWP, auto simp: pred_defs)
+  then show ?thesis by (intro false_wp, auto simp: assert_def)
 qed 
 
-subsection \<open>Rewrite Introduction Rules\<close>
-
-text \<open>Skip Rewrite Rule\<close>
-lemma skipRW:
-  assumes "R,G \<turnstile>\<^sub>w P \<ge> Q" 
-  shows "R,G \<turnstile>\<^sub>w P {Skip} Q"
-  using rewriteWP[OF skip_wp assms] .
-
-text \<open>If Rewrite Rule\<close>
-lemma ifRW:
-  assumes "R,G \<turnstile>\<^sub>w P \<ge> (wp\<^sub>i (cmp e\<^sub>1 f e\<^sub>2) P\<^sub>1 \<and>\<^sub>p wp\<^sub>i (ncmp e\<^sub>1 f e\<^sub>2) P\<^sub>2)"
-  assumes "R,G \<turnstile>\<^sub>w P\<^sub>1 {c\<^sub>1} Q"
-  assumes "R,G \<turnstile>\<^sub>w P\<^sub>2 {c\<^sub>2} Q"
-  shows "R,G \<turnstile>\<^sub>w P {If e\<^sub>1 f e\<^sub>2 c\<^sub>1 c\<^sub>2} Q"
-  using rewriteWP[OF ifWP[OF assms(2,3)] assms(1)] . 
-
-text \<open>While Rewrite Rule\<close>
-lemma whileRW:
-  assumes order: "R,G \<turnstile>\<^sub>w N \<ge> stabilize R I"
-  assumes recur: "R,G \<turnstile>\<^sub>w P {c} stabilize R I"
-  assumes side: "I \<turnstile>\<^sub>p wp\<^sub>i (cmp e\<^sub>1 f e\<^sub>2) P \<and>\<^sub>p wp\<^sub>i (ncmp e\<^sub>1 f e\<^sub>2) Q"
-  shows "R,G \<turnstile>\<^sub>w N {While e\<^sub>1 f e\<^sub>2 I c} Q"
-  using rewriteWP[OF whileWP[OF side recur] order] .
-
-text \<open>Do While Rewrite Rule\<close>
-lemma doWhileRW:
-  assumes order: "R,G \<turnstile>\<^sub>w P \<ge> stabilize R I"
-  assumes recur: "R,G \<turnstile>\<^sub>w stabilize R I {c} (wp\<^sub>i (cmp e\<^sub>1 f e\<^sub>2) (stabilize R I) \<and>\<^sub>p wp\<^sub>i (ncmp e\<^sub>1 f e\<^sub>2) Q)"
-  shows "R,G \<turnstile>\<^sub>w P {DoWhile I c e\<^sub>1 f e\<^sub>2} Q"
-  using rewriteWP[OF doWhileWP[OF recur] order] .
-
-subsection \<open>Soundness\<close>
-
-lemma wellformed_assert [intro]:
-  assumes "wellformed R G Q"
-  shows "wellformed R G (assert p)"
-  using assms by (auto simp: wellformed_def assert_def stable_def)
-
-lemma wellformed_wp [intro]:
-  assumes "wellformed R G Q"
-  shows "wellformed R G (ARMv8_Rules.wp R G c Q)"
-  sorry (*
-  using assms by (induct c arbitrary: Q) fastforce+
-*)
-
-lemma wp_valid:
-  shows "R,G \<turnstile>\<^sub>w wp R G c Q {c} Q" 
+text \<open>Com Rule\<close>
+theorem com_wp:
+  shows "R,G,I \<turnstile>\<^sub>w wp R c Q {c} Q" 
 proof (induct c arbitrary: Q)
-  case Skip
-  thus ?case using skip_wp by auto
-next
   case Fence
-  thus ?case using fence_sound by (auto simp: valid_def)
+  thus ?case unfolding valid_def lift\<^sub>c.simps by (intro conjI impI basic_wp\<^sub>i_local) auto
 next
-  case (Load)
-  thus ?case using load_sound by (auto simp: valid_def) 
-next
-  case (Store)
-  thus ?case using store_sound by (auto simp: valid_def) 
-next
-  case (Op)
-  thus ?case using op_sound by (auto simp: valid_def)
-next
-  case (Seq c\<^sub>1 c\<^sub>2)
-  thus ?case using seq_wp unfolding wp.simps by blast
-next
-  case (If f r c\<^sub>1 c\<^sub>2)
-  thus ?case using ifWP unfolding wp.simps by blast
-next
-  case (While f r I c)
-  thus ?case unfolding wp.simps
-    by (intro assertWP impI whileRW) (auto simp add: pred_defs)
-next
-  case (DoWhile I c e\<^sub>1 f e\<^sub>2)
-  thus ?case unfolding wp.simps
-    by (intro assertWP impI doWhileRW ord_refl; rule rewriteWP) (blast intro: ord_stabilize)+
+  case (Op r e)
+  thus ?case unfolding valid_def lift\<^sub>c.simps 
+    by (intro conjI impI basic_wp\<^sub>i_local) (auto simp: rg_upd_def)
 next
   case (Test p)
-  thus ?case using test_sound by (auto simp: valid_def)
+  thus ?case unfolding valid_def lift\<^sub>c.simps
+    by (intro conjI impI rules.basic)
+       (auto simp: atomic_rule_def wp_def pred_defs guar_def step_def elim!: stabilizeE)
 next
   case (Assert p)
-  thus ?case using assert_sound by (auto simp: valid_def)
+  thus ?case unfolding valid_def lift\<^sub>c.simps
+    by (intro conjI impI rules.basic)
+       (auto simp: atomic_rule_def wp_def pred_defs guar_def step_def elim!: stabilizeE)
 next
-  case (CAS)
-  thus ?case using cas_sound by (auto simp: valid_def)
-qed
+  case (Load c r\<^sub>a r a)
+  thus ?case unfolding valid_def by (intro conjI impI, force) (expand_seq, basic_wp\<^sub>i+)
+next
+  case (Store c r\<^sub>a r a)
+  thus ?case unfolding valid_def by (intro conjI impI, force) (expand_seq, basic_wp\<^sub>i+)
+next
+  case (CAS c r\<^sub>a r\<^sub>1 r\<^sub>2 r T F a)
+  thus ?case unfolding valid_def by (intro conjI impI, force) (expand_seq, basic_wp\<^sub>i+)
+next
+  case (If b c\<^sub>1 c\<^sub>2)
+  thus ?case unfolding wp.simps by (blast intro: if_wp)
+next
+  case (While b I c)
+  thus ?case unfolding wp.simps by (intro assert_wp impI while_wp) (auto simp: pred_defs)
+next
+  case (DoWhile I c b)
+  thus ?case unfolding wp.simps by (intro assert_wp do_wp; rule rewrite_wp) auto
+qed (auto simp: valid_def)
+
+subsection \<open>High-Level Theorem\<close>
 
 text \<open>Soundness lemma for WP reasoning over ARMv8\<close>
 theorem armv8_wp_sound:
   assumes wf: "transitive R" "reflexive R" "reflexive G" 
-  assumes st: "stable (step\<^sub>R R) (Collect Q)" 
-  assumes g: "guar\<^sub>c c G"
-  assumes P: "P \<turnstile>\<^sub>p wp R G c Q"
-  assumes i: "inter (step\<^sub>R R) (step G) (lift\<^sub>c c)" (* Rephrase this in terms of the ARMv8 analysis *)
-  shows "\<Turnstile> c SAT [P, R, G, Q]"
+  assumes st: "stable\<^sub>t R Q" 
+  assumes g: "guar\<^sub>c c (inv I \<and>\<^sub>p G)"
+  assumes P: "P \<turnstile>\<^sub>p wp R c Q"
+  shows "\<Turnstile> c SAT [P, R, G, Q, I]"
 proof -
-  have "wellformed R G Q" using wf st by (auto simp: wellformed_def)
-  hence "R,G \<turnstile>\<^sub>s wp R G c Q {c} Q" using g wp_valid unfolding valid_def by blast
-  hence "R,G \<turnstile>\<^sub>s P {c} Q" by (rule rules.conseq) (insert P, auto simp: entail_def)
-  thus ?thesis using i by (intro sound thread) auto
+  have "R,G,I \<turnstile>\<^sub>s wp R c Q {c} Q" using wf st g com_wp unfolding valid_def by blast
+  hence "R,G,I \<turnstile>\<^sub>s P {c} Q" by (rule rules.conseq) (insert P, auto)
+  thus ?thesis by (intro sound thread) auto
 qed
 
 end
