ARMv8_State.thy
@@ -2,37 +2,41 @@ theory ARMv8_State
   imports Main
 begin
 
-
 section \<open>State Encoding\<close>
 
-record 'v gstate = st :: "'v \<Rightarrow> 'v"
-record ('v,'r) tstate = "'v gstate" + rg :: "'r \<Rightarrow> 'v"
-type_synonym ('v,'r,'a) pred = "('v,'r,'a) tstate_scheme \<Rightarrow> bool"
-type_synonym ('v,'a) rpred = "(('v,'a) gstate_scheme \<times> ('v,'a) gstate_scheme) \<Rightarrow> bool"
+record 'v gstate_rec = st :: "'v \<Rightarrow> 'v"
+record ('v,'r) tstate_rec = "'v gstate_rec" + rg :: "'r \<Rightarrow> 'v"
 
+type_synonym ('v,'r,'a) tstate = "('v,'r,'a) tstate_rec_scheme"
+type_synonym ('v,'a) gstate = "('v,'a) gstate_rec_scheme"
 
+type_synonym ('v,'r,'a) pred = "('v,'r,'a) tstate \<Rightarrow> bool"
+type_synonym ('v,'a) gpred = "('v,'a) gstate \<Rightarrow> bool"
 
-(*
-type_synonym ('v) global = "(('v \<Rightarrow> 'v))"
-type_synonym ('v,'r) state = "(('v) global \<times> ('r \<Rightarrow> 'v))"
-type_synonym ('v,'r) rpred = "(('v) global \<times> ('v) global) \<Rightarrow> bool"
-type_synonym ('v,'r) gpred  = "('v) global \<Rightarrow> bool"
-*)
+type_synonym ('v,'r,'a) trel = "(('v,'r,'a) tstate \<times> ('v,'r,'a) tstate) \<Rightarrow> bool"
+type_synonym ('v,'a) grel = "(('v,'a) gstate \<times> ('v,'a) gstate) \<Rightarrow> bool"
+type_synonym ('v,'r,'a) trans = "('v,'r,'a) pred \<Rightarrow> ('v,'r,'a) pred"
+type_synonym ('v,'r,'a) rtrans = "('v,'r,'a) trel \<Rightarrow> ('v,'r,'a) trel"
 
+type_synonym ('v,'r,'a) auxfn = "('v,'r,'a) tstate \<Rightarrow> 'a"
 
 section \<open>Write Operations\<close>
 
-definition st_upd :: "(('v,'a) gstate_scheme) \<Rightarrow> 'v \<Rightarrow> 'v \<Rightarrow> (('v,'a) gstate_scheme)"
-  where "st_upd f a b = f \<lparr> st := ((st f) (a := b)) \<rparr>"
+definition st_upd :: "('v,'a) gstate \<Rightarrow> 'v \<Rightarrow> 'v \<Rightarrow> ('v,'a) gstate"
+  where "st_upd m a b = m \<lparr> st := ((st m) (a := b)) \<rparr>"
 
-definition rg_upd :: "(('v,'r,'a) tstate_scheme) \<Rightarrow> 'r \<Rightarrow> 'v \<Rightarrow> (('v,'r,'a) tstate_scheme)"
-  where "rg_upd f a b = f \<lparr> rg := ((rg f) (a := b)) \<rparr>"
+definition rg_upd :: "('v,'r,'a) tstate \<Rightarrow> 'r \<Rightarrow> 'v \<Rightarrow> ('v,'r,'a) tstate"
+  where "rg_upd m a b = m \<lparr> rg := ((rg m) (a := b)) \<rparr>"
+
+definition aux_upd :: "('v,'r,'a) tstate \<Rightarrow> ('v,'r,'a) auxfn \<Rightarrow> ('v,'r,'a) tstate"
+  where "aux_upd m f \<equiv> m\<lparr>tstate_rec.more := f m\<rparr>"
 
 nonterminal updbinds and updbind
 
 syntax
-  "_updbindm" :: "'a \<Rightarrow> 'a \<Rightarrow> updbind"             ("(2_ :=\<^sub>s/ _)")
-  "_updbindr" :: "'a \<Rightarrow> 'a \<Rightarrow> updbind"             ("(2_ :=\<^sub>r/ _)")
+  "_updbindm" :: "'a \<Rightarrow> 'a \<Rightarrow> updbind"            ("(2_ :=\<^sub>s/ _)")
+  "_updbindr" :: "'a \<Rightarrow> 'a \<Rightarrow> updbind"            ("(2_ :=\<^sub>r/ _)")
+  "_updbinda" :: "'a \<Rightarrow> updbind"                  ("(2aux:/ _)")
   ""         :: "updbind \<Rightarrow> updbinds"             ("_")
   "_updbinds":: "updbind \<Rightarrow> updbinds \<Rightarrow> updbinds" ("_,/ _")
   "_Update"  :: "'a \<Rightarrow> updbinds \<Rightarrow> 'a"            ("_/'((_)')" [1000, 0] 900)
@@ -41,31 +45,39 @@ translations
   "_Update f (_updbinds b bs)" \<rightleftharpoons> "_Update (_Update f b) bs"
   "f(x:=\<^sub>ry)" \<rightleftharpoons> "CONST rg_upd f x y"
   "f(x:=\<^sub>sy)" \<rightleftharpoons> "CONST st_upd f x y"
+  "f(aux: y)" \<rightleftharpoons> "CONST aux_upd f y"
+
+definition glb :: "('v,'r,'a) tstate \<Rightarrow> ('v,'a) gstate"
+  where "glb m \<equiv> \<lparr> st = st m, \<dots> = more m \<rparr>"
+
+definition set_glb :: "('v,'r,'a) tstate \<Rightarrow> ('v,'a) gstate \<Rightarrow> ('v,'r,'a) tstate"
+  where "set_glb m g \<equiv> \<lparr> st = st g, rg = rg m, \<dots> = gstate_rec.more g \<rparr>"
+
+lemma [simp]:
+  "set_glb m (glb m) = m"
+  by (auto simp: set_glb_def glb_def)
 
 section \<open>Simple Predicate Encoding\<close>
 
 named_theorems pred_defs
 
-definition conj  (infixr "\<and>\<^sub>p" 35)
+abbreviation conj  (infixr "\<and>\<^sub>p" 35)
   where "conj l r \<equiv> \<lambda>m. (l m) \<and> (r m)"
 
-definition disj  (infixr "\<or>\<^sub>p" 35)
+abbreviation disj  (infixr "\<or>\<^sub>p" 35)
   where "disj l r \<equiv> \<lambda>m. (l m) \<or> (r m)"
 
-definition imp  (infixr "\<longrightarrow>\<^sub>p" 35)
+abbreviation imp  (infixr "\<longrightarrow>\<^sub>p" 35)
   where "imp l r \<equiv> \<lambda>m. (l m) \<longrightarrow> (r m)"
 
-definition entail (infix "\<turnstile>\<^sub>p" 25)
+abbreviation entail (infix "\<turnstile>\<^sub>p" 25)
   where "entail P Q \<equiv> \<forall>m. P m \<longrightarrow> Q m"
 
 definition assert
   where "assert b \<equiv> \<lambda>m. b"
 
-declare conj_def [pred_defs]
-declare disj_def [pred_defs]
-declare imp_def [pred_defs]
-declare assert_def [pred_defs]
-declare entail_def [pred_defs]
+abbreviation True\<^sub>p
+  where "True\<^sub>p \<equiv> \<lambda>m. True"
 
 lemma [simp]:
   "(P \<turnstile>\<^sub>p P) = True"
@@ -82,5 +94,62 @@ definition reflexive
 
 definition transitive 
   where "transitive R \<equiv> \<forall>m m' m''. R (m,m') \<longrightarrow> R (m',m'') \<longrightarrow> R (m,m'')"
+
+definition stabilize :: "('v,'a) grel \<Rightarrow> ('v,'r,'a) pred \<Rightarrow> ('v,'r,'a) pred"
+  where "stabilize R P \<equiv> \<lambda>m. \<forall>g. R (glb m,g) \<longrightarrow> P (set_glb m g)"
+
+section \<open>Simp\<close>
+
+lemma [simp]:
+  "rg (set_glb m g) r\<^sub>a = rg m r\<^sub>a"
+  by (auto simp: set_glb_def)
+
+lemma [simp]:
+  "set_glb (set_glb m g) g' = set_glb m g'"
+  by (auto simp: set_glb_def)
+
+lemma [simp]:
+  "set_glb (m\<lparr>tstate_rec.more := a\<rparr>) g = set_glb m g"
+  by (auto simp: set_glb_def)
+
+lemma [simp]:
+  "st (set_glb m g) = st g"
+  by (auto simp: set_glb_def)
+
+lemma [simp]:
+  "\<forall>m. \<not> P m \<Longrightarrow> Collect P = {}"
+  by (auto)
+
+lemma [simp]:
+  "glb (m\<lparr>rg := e\<rparr>) = glb m"
+  unfolding glb_def by auto
+
+lemma [simp]:
+  "m(r :=\<^sub>r e)\<lparr>tstate_rec.more := a\<rparr> = (m\<lparr>tstate_rec.more := a\<rparr>)(r :=\<^sub>r e)"
+  by (auto simp: rg_upd_def)
+
+lemma [simp]:
+  "glb (m(r :=\<^sub>r T)) = glb m"
+  by (auto simp: glb_def rg_upd_def)
+
+lemma [simp]:
+  "m(aux: tstate_rec.more) = m"
+  by (auto simp: aux_upd_def)
+
+lemma [simp]:
+  "glb (set_glb m g) = g"
+  by (auto simp: glb_def set_glb_def)
+
+lemma [simp]:
+  "glb (x(x3 :=\<^sub>r e, aux: x4)) = glb (x(aux: \<lambda>m. x4 (m(x3 :=\<^sub>r e))))"
+  by (auto simp: rg_upd_def aux_upd_def glb_def)
+
+lemma [intro]:
+  "reflexive G \<Longrightarrow> G (m,m)"
+  by (auto simp: reflexive_def)
+
+lemma entail_refl [intro]:
+  "P \<turnstile>\<^sub>p P"
+  by (auto simp: pred_defs)
 
 end
