Rules.thy
@@ -19,8 +19,8 @@ inductive rules :: "'b rpred \<Rightarrow> 'b rpred \<Rightarrow> 'b set \<Right
   where
   basic[intro]:  "R,G \<turnstile>\<^sub>A P {\<alpha>} Q \<Longrightarrow> R,G \<turnstile> P { Basic \<alpha> } Q" |
   nil[intro]:    "stable R P \<Longrightarrow> R,G \<turnstile> P { Nil } P" |
-  seq[intro]:    "R,G \<turnstile> P { c\<^sub>1 } Q \<Longrightarrow> R,G \<turnstile> Q { c\<^sub>2 } M \<Longrightarrow> R,G \<turnstile> P { c\<^sub>1 ;; c\<^sub>2 } M" |
-  ord[intro]:    "R,G \<turnstile> P { c\<^sub>1 } Q \<Longrightarrow> R,G \<turnstile> Q { c\<^sub>2 } M \<Longrightarrow> R,G \<turnstile> P { c\<^sub>1 \<cdot> c\<^sub>2 } M" |
+  seq[intro]:    "R,G \<turnstile> Q { c\<^sub>2 } M \<Longrightarrow> R,G \<turnstile> P { c\<^sub>1 } Q \<Longrightarrow> R,G \<turnstile> P { c\<^sub>1 ;; c\<^sub>2 } M" |
+  ord[intro]:    "R,G \<turnstile> Q { c\<^sub>2 } M \<Longrightarrow> R,G \<turnstile> P { c\<^sub>1 } Q \<Longrightarrow> R,G \<turnstile> P { c\<^sub>1 \<cdot> c\<^sub>2 } M" |
   choice[intro]: "R,G \<turnstile> P { c\<^sub>1 } Q \<Longrightarrow> R,G \<turnstile> P { c\<^sub>2 } Q \<Longrightarrow> R,G \<turnstile> P { c\<^sub>1 \<sqinter> c\<^sub>2 } Q" |
   seqset[intro]: "\<forall>s \<in> S. R,G \<turnstile> P { seq2com s } Q \<Longrightarrow> R,G \<turnstile> P { \<Sqinter> S } Q" |
   loop[intro]:   "stable R P \<Longrightarrow> R,G \<turnstile> P { c } P \<Longrightarrow> R,G \<turnstile> P { c* } P" |
@@ -156,6 +156,10 @@ next
   case (SeqChoice x)
   thus ?case by (intro ballI seqset false_seqI) auto
 qed auto
+
+lemma seq_rot:
+  "R,G \<turnstile> P { c\<^sub>1 } Q \<Longrightarrow> R,G \<turnstile> Q { c\<^sub>2 } M \<Longrightarrow> R,G \<turnstile> P { c\<^sub>1 ;; c\<^sub>2 } M" 
+  by auto
 
 end
 
